Forgot to add file

theories/L6_PCPS/logical_relations.v
@@ -1,8 +1,1697 @@
 Require Import Coq.NArith.BinNat Coq.Relations.Relations Coq.MSets.MSets Coq.MSets.MSetRBT
         Coq.Lists.List Coq.omega.Omega Coq.Sets.Ensembles.
-Require Import cps cps_util identifiers env eval ctx Ensembles_util List_util.
+Require Import cps eval cps_util identifiers env ctx Ensembles_util List_util.
 Import ListNotations.
 
+
+Section Log_rel.
+
+  Variable (pr : prims).
+
+  (** step-indexed preorder on cps terms *)
+  (* Expression relation : 
+   * ---------------------
+   *  (e1, ρ1) ~_k (e2, ρ2) iff 
+   *    forall c1 <= k, 
+   *      ρ1 |- e1 ->^c1 v1 -> 
+   *      exists v2, p2 |- e2 -> v2 /\ v1 ~_(k-c1) v2 
+   * Value relation :
+   * ----------------
+   * Integers: (n1 ~_k n2) iff n1 = n2
+   * Constructors: [v_1, .., v_n] ~_k [v'_1, .., v'_m] iff
+                     n <= m /\ v_1 ~_k v'_1 /\ ... /\ v_n ~_k v'_n'
+   * Closures: (\f1 x1. e1, ρ1) ~_k (\f2 x2. e2, ρ2) iff 
+   *              \forall v1 v2 i < k, v1 ~_j v2 => 
+   *                (e1, ρ1[x1 -> v1, f1 -> (\f1 x1. e1, ρ1)]) ~_j 
+   *                (e2, ρ2[x2 -> v2, f2 -> (\f2 x2. e2, ρ2)])
+   *)
+  Fixpoint preord_val (k : nat) (v1 v2 : val) {struct k} : Prop :=
+    let preord_exp (k : nat) (p1 p2 : exp * env) : Prop :=
+        let '(e1, rho1) := p1 in
+        let '(e2, rho2) := p2 in
+        forall v1 c1,
+           c1 <= k -> bstep_e pr rho1 e1 v1 c1 ->
+           exists v2 c2, bstep_e pr rho2 e2 v2 c2 /\ 
+                    preord_val (k - c1) v1 v2
+    in
+    let fix preord_val_aux (v1 v2 : val) {struct v1} : Prop :=
+        let fix Forall2_aux vs1 vs2 :=
+            match vs1, vs2 with
+              | [], _ => True
+              | v1 :: vs1, v2 :: vs2 =>
+                preord_val_aux v1 v2 /\ Forall2_aux vs1 vs2
+              | _, _ => False
+            end
+        in
+        match v1, v2 with
+          | Vfun rho1 defs1 f1, Vfun rho2 defs2 f2 =>
+            forall (vs1 vs2 : list val) (j : nat) (t1 : type) 
+              (xs1 : list var) (e1 : exp) (rho1' : env),
+              length vs1 = length vs2 ->
+              find_def f1 defs1 = Some (t1, xs1, e1) ->
+              Some rho1' = setlist xs1 vs1 (def_funs defs1 defs1 rho1 rho1) ->
+              exists (t2 : type) (xs2 : list var) (e2 : exp) (rho2' : env),
+                find_def f2 defs2 = Some (t2, xs2, e2) /\
+                Some rho2' = setlist xs2 vs2 (def_funs defs2 defs2 rho2 rho2) /\
+                match k with
+                  | 0 => True
+                  | S k =>
+                    let R := preord_val (k - (k-j)) in
+                    j < S k ->
+                    Forall2 R vs1 vs2 ->
+                    preord_exp (k - (k-j)) (e1, rho1') (e2, rho2')
+                end
+          | Vconstr tau1 t1 vs1, Vconstr tau2 t2 vs2 =>
+            t1 = t2 /\ Forall2_aux vs1 vs2
+          | Vint n1, Vint n2 => n1 = n2
+          | _, _ => False
+        end
+    in preord_val_aux v1 v2.
+           
+  Definition preord_exp (k : nat) (p1 p2 : exp * env) : Prop :=
+    let '(e1, rho1) := p1 in
+    let '(e2, rho2) := p2 in
+    forall v1 c1,
+      c1 <= k -> bstep_e pr rho1 e1 v1 c1 ->
+      exists v2 c2, bstep_e pr rho2 e2 v2 c2 /\
+               preord_val (k - c1) v1 v2.
+
+  (** more compact definition of the value preorder *)
+  Definition preord_val' (k : nat) (v1 v2 : val) : Prop :=
+    match v1, v2 with
+      | Vfun rho1 defs1 f1, Vfun rho2 defs2 f2 =>
+        forall (vs1 vs2 : list val) j (t1 : type) (xs1 : list var)
+               (e1 : exp) (rho1' : env),
+          length vs1 = length vs2 -> 
+          find_def f1 defs1 = Some (t1, xs1, e1) ->
+          Some rho1' = setlist xs1 vs1 (def_funs defs1 defs1 rho1 rho1) ->
+          exists (t2 : type) (xs2 : list var) (e2 : exp) (rho2' : env),
+            find_def f2 defs2 = Some (t2, xs2, e2) /\
+            Some rho2' = setlist xs2 vs2 (def_funs defs2 defs2 rho2 rho2) /\
+            (j < k -> Forall2 (preord_val j) vs1 vs2 ->
+             preord_exp j (e1, rho1') (e2, rho2'))
+      | Vconstr tau1 t1 vs1, Vconstr tau2 t2 vs2 =>
+        t1 = t2 /\ Forall2_asym (preord_val k) vs1 vs2
+      | Vint n1, Vint n2 => n1 = n2
+      | _, _ => False
+    end.
+
+  (** correspondence of the two definitions *)
+  Lemma preord_val_eq (k : nat) (v1 v2 : val) :
+    preord_val k v1 v2 <-> preord_val' k v1 v2.
+  Proof.
+    destruct k as [ | k ]; destruct v1; destruct v2;
+    eauto; try (split; intros H; (now simpl in H; inv H)).
+    - split.
+      * revert l0; induction l as [| x xs IHxs];
+        intros l2; destruct l2 as [| y ys ];
+        try (now intros [H1 H2]; split; eauto; inv H2).
+        intros H; split; destruct H as [H1 [H2 H3]]; eauto.
+        constructor; [ now eauto | now eapply IHxs ].
+      * revert l0; induction l as [| x xs IHxs];
+        intros l2; destruct l2 as [| y ys ];
+        try (now intros [H1 H2]; split; eauto; inv H2).
+        intros H; split; inv H; eauto. inv H1.
+        split; [ now eauto | now eapply IHxs ].
+    - split; intros Hpre; simpl; intros; 
+      edestruct (Hpre vs1 vs2 0) as [t2 [xs2 [e2 [rho' [H1' [H2' H3']]]]]];
+      eauto; do 4 eexists; repeat split; eauto; intros Hc; exfalso; omega.
+    - revert l0; induction l as [| x xs IHxs];
+      intros l2; destruct l2 as [| y ys ];
+      split; intros H; try (now simpl in H; inv H); try now (simpl; eauto).
+      + destruct H as [Heq [H1 H2]]; subst.  
+        constructor; eauto. constructor; eauto. eapply IHxs.
+        constructor; eauto.
+      + inv H. inv H1. split. reflexivity.
+        split. now eauto. eapply IHxs. split; eauto. 
+    - split; intros Hpre; simpl; intros; 
+      now (edestruct Hpre as [t2 [xs2 [e2 [rho' [H1' [H2' H3']]]]]]; eauto;
+           do 4 eexists; do 2 (split; eauto); intros Hleq Hf v1 c1 Hleq' Hstep;
+           (assert (Heq : k - (k - j) = j) by omega); rewrite Heq in *;
+           eapply H3'; eauto).
+  Qed.
+
+  Opaque preord_val.
+  
+  (** Environment relation for a single point (i.e. variable) : 
+    * ρ1 ~_k^x ρ2 iff ρ1(x) = Some v -> ρ2(x) = Some v' /\ v ~_k v' *)
+  Definition preord_var_env (k : nat) (rho1 rho2 : env) (x y : var) : Prop :=
+    forall v1, 
+      M.get x rho1 = Some v1 -> 
+      exists v2, M.get y rho2 = Some v2 /\ preord_val k v1 v2.
+    
+  (** Environment relation for a set of points (i.e. predicate over variables) : 
+    * ρ1 ~_k^S ρ2 iff 
+    *   forall x, S x -> ρ1(x) = Some v -> ρ2(x) = Some v' /\ v ~_k v' *)
+  Definition preord_env_P (P : Ensemble var) k rho1 rho2 :=
+    forall (x : var), P x -> preord_var_env k rho1 rho2 x x.
+
+  (** Environment relation for the whole domain of definition :
+    * ρ1 ~_k ρ2 iff forall x, ρ1(x) = v => ρ2(x) = v' /\ v ~_k v' *)
+  Definition preord_env (k : nat) (rho1 rho2 : env) : Prop :=
+    preord_env_P (fun _ => True) k rho1 rho2.
+  
+  Open Scope ctx_scope.
+
+  (** Context relation. *)
+  Definition preord_ctx (k : nat) (rho1 rho2 : env)
+             (p1 p2 : exp_ctx * env) :=
+    let '(c1, rho1') := p1 in
+    let '(c2, rho2') := p2 in
+    forall e1 e2, preord_exp k (e1, rho1) (e2, rho2) ->
+                  preord_exp k (c1 |[ e1 ]|, rho1')
+                             (c2 |[ e2 ]|, rho2').
+
+  (** Lemmas about extending the environment *)
+  Lemma preord_var_env_extend_eq :
+    forall (rho1 rho2 : env) (k : nat) (x : var) (v1 v2 : val),
+      preord_val k v1 v2 ->
+      preord_var_env k (M.set x v1 rho1) (M.set x v2 rho2) x x.
+  Proof.
+    intros rho1 rho2 k x v1 v2 Hval x' Hget.
+    rewrite M.gss in Hget. inv Hget. eexists. rewrite M.gss. split; eauto.
+  Qed.
+  
+  Lemma preord_var_env_extend_neq :
+    forall (rho1 rho2 : env) (k : nat) (x y : var) (v1 v2 : val),
+      preord_var_env k rho1 rho2 y y ->
+      y <> x ->
+      preord_var_env k (M.set x v1 rho1) (M.set x v2 rho2) y y.
+  Proof.
+    intros rho1 rho2 k x  y v1 v2 Hval Hneq x' Hget.
+    rewrite M.gso in *; eauto.
+  Qed.
+
+  Lemma preord_var_env_extend :
+    forall (rho1 rho2 : env) (k : nat) (x y : var) (v1 v2 : val),
+      preord_var_env k rho1 rho2 y y ->
+      preord_val k v1 v2 ->
+      preord_var_env k (M.set x v1 rho1) (M.set x v2 rho2) y y.
+  Proof.
+    intros rho1 rho2 k x y v1 v2 Henv Hval.
+    destruct (Coqlib.peq y x); subst.
+    - apply preord_var_env_extend_eq; eauto.
+    - apply preord_var_env_extend_neq; eauto.
+  Qed.
+
+  (** The environment relation is antimonotonic in the set
+    * of free variables *) 
+  Lemma preord_env_P_antimon (P1 P2 : var -> Prop) k rho1 rho2 :
+    preord_env_P P2 k rho1 rho2 ->
+    (Included var P1 P2) ->
+    preord_env_P P1 k rho1 rho2.
+  Proof.
+    intros Hpre Hin x HP2. eapply Hpre; eapply Hin; eauto.
+  Qed.
+
+  Global Instance preord_env_proper  :
+    Proper (Same_set var ==> Logic.eq ==> Logic.eq ==> Logic.eq ==> iff)
+           preord_env_P.
+  Proof.
+    intros s1 s2 [H1 H2]; split; intros Hpre;
+    eapply preord_env_P_antimon; subst; eauto.
+  Qed.
+
+  (** Lemmas about the sets that index the environment relation *)
+  Lemma preord_env_Empty_set k (rho1 rho2 : env) :
+    preord_env_P (Empty_set var) k rho1 rho2.
+  Proof.
+    intros x H. inv H.
+  Qed.
+  
+  Lemma preord_env_P_union (P1 P2 : var -> Prop) k rho1 rho2 :
+    preord_env_P P1 k rho1 rho2 ->
+    preord_env_P P2 k rho1 rho2 ->
+    preord_env_P (Union var P1 P2) k rho1 rho2.
+  Proof.
+    intros Hpre1 Hpre2 x HP2. inv HP2; eauto.
+  Qed.
+
+  Lemma preord_env_P_inter_l (P1 P2 : var -> Prop) k rho1 rho2 :
+    preord_env_P P1 k rho1 rho2 ->
+    preord_env_P (Intersection var P1 P2) k rho1 rho2.
+  Proof.
+    intros Hpre x HP2. inv HP2; eauto.
+  Qed.
+
+  Lemma preord_env_P_inter_r (P1 P2 : var -> Prop) k rho1 rho2 :
+    preord_env_P P2 k rho1 rho2 ->
+    preord_env_P (Intersection var P1 P2) k rho1 rho2.
+  Proof.
+    intros Hpre x HP2.
+    inv HP2; eauto.
+  Qed.
+
+  (** Extend the related environments with a single point *)
+  Lemma preord_env_P_extend :
+    forall P (rho1 rho2 : env) (k : nat) (x : var) (v1 v2 : val),
+      preord_env_P (Setminus var P (Singleton var x)) k rho1 rho2 ->
+      preord_val k v1 v2 ->
+      preord_env_P P k (M.set x v1 rho1) (M.set x v2 rho2).
+  Proof.
+    intros P rho1 rho2 k x v1 v2 Henv Hval x' HP v1' Hget.
+    rewrite M.gsspec in Hget. destruct (Coqlib.peq x' x); subst.
+    - inv Hget. eexists. rewrite M.gss. split; eauto.
+    - apply Henv in Hget; eauto. destruct Hget as [v2' [Heq Hpre]].
+      eexists; split; eauto. rewrite M.gso; eauto. constructor; eauto.
+      intros Hin. inv Hin. congruence.
+  Qed.
+
+  (** Extend the related environments with a list *)
+  Lemma preord_env_P_setlist_l:
+    forall (P1 P2 : var -> Prop) (rho1 rho2 rho1' rho2' : env)
+      (k : nat) (xs : list var) (vs1 vs2 : list val),
+      preord_env_P P1 k rho1 rho2 ->
+      (forall x, ~ List.In x xs -> P2 x -> P1 x) ->
+      Forall2 (preord_val k) vs1 vs2 ->
+      setlist xs vs1 rho1 = Some rho1' ->
+      setlist xs vs2 rho2 = Some rho2' ->
+      preord_env_P P2 k rho1' rho2'.
+  Proof. 
+    intros P1 P2 rho1' rho2' rho1 rho2 k xs vs1 vs2 Hpre Hyp Hall Hset1 Hset2
+           x HP v Hget.
+    destruct (in_dec var_dec x xs).
+    - edestruct setlist_Forall2_get as [v1 [v2 [Hget1 [Hget2 HP']]]]; eauto.
+      rewrite Hget in Hget1. inv Hget1. repeat eexists; eauto.
+    - erewrite <- setlist_not_In in Hget; eauto.
+      edestruct Hpre as [v2 [Hget' Hpre']]; eauto.
+      repeat eexists; eauto. erewrite <- setlist_not_In; eauto.
+  Qed.
+
+  
+  Lemma preord_var_env_getlist (rho1 rho2 : env) (k : nat)
+        (xs ys : list var) (vs1 : list val) :
+    Forall2 (preord_var_env k rho1 rho2) xs ys ->
+    getlist xs rho1 = Some vs1 ->
+    exists vs2,
+      getlist ys rho2 = Some vs2 /\ Forall2 (preord_val k) vs1 vs2.
+  Proof.
+    revert ys vs1. induction xs as [| x xs IHxs]; intros ys vs2 Hall Hget.
+    - destruct ys; inv Hall. inv Hget. eexists. split; simpl; eauto.
+    - simpl in Hget.
+      destruct (M.get x rho1) eqn:Heq1; try discriminate.
+      destruct (getlist xs rho1) eqn:Heq2; try discriminate. inv Hget.
+      destruct ys as [| y ys]; inv Hall. 
+      destruct (IHxs ys l H4 eq_refl) as [vs2 [Hget HAll]].
+      destruct (H2 _ Heq1) as [v2 [Heq Hpre]].
+      eexists. split; simpl; eauto. rewrite Hget, Heq. eauto.
+  Qed.
+
+  Lemma preord_env_P_getlist_l (P : var -> Prop) (rho1 rho2 : env) (k : nat)
+        (xs : list var) (vs1 : list val) :
+    preord_env_P P k rho1 rho2 ->
+    Included _ (FromList xs) P ->
+    getlist xs rho1 = Some vs1 ->
+    exists vs2,
+      getlist xs rho2 = Some vs2 /\ Forall2 (preord_val k) vs1 vs2.
+  Proof.
+    intros Henv. revert vs1.
+    induction xs as [| x xs IHxs]; intros vs1 Hp Hget.
+    - inv Hget. eexists. split; simpl; eauto.
+    - simpl in Hget. destruct (M.get x rho1) eqn:Heq1; try discriminate.
+      destruct (getlist xs rho1) eqn:Heq2; try discriminate. inv Hget.
+      edestruct (IHxs l) as  [vs2 [Hget HAll]]; eauto.
+      + intros x' Hin. eapply Hp. constructor 2; eauto.
+      + eapply Henv in Heq1. destruct Heq1 as [v2 [H1 H2]].
+        eexists. split; simpl; eauto. rewrite H1. rewrite Hget.
+        constructor. apply Hp. now constructor.
+  Qed.
+  
+  Corollary preord_env_getlist_l (rho1 rho2 : env) (k : nat)
+        (xs : list var) (vs1 : list val) :
+    preord_env k rho1 rho2 ->
+    getlist xs rho1 = Some vs1 ->
+    exists vs2,
+      getlist xs rho2 = Some vs2 /\ Forall2 (preord_val k) vs1 vs2.
+  Proof.
+    intros. eapply preord_env_P_getlist_l; eauto.
+    intros x H'; simpl; eauto.
+  Qed.
+
+  Corollary preord_env_extend (rho1 rho2 : env) (k : nat)
+        (x : var) (v1 v2 : val) :
+    preord_env k rho1 rho2 ->
+    preord_val k v1 v2 ->
+    preord_env k (M.set x v1 rho1) (M.set x v2 rho2).
+  Proof.
+    intros H1 Hval. apply preord_env_P_extend; eauto.
+    eapply preord_env_P_antimon; eauto. intros x' H; simpl; eauto.
+  Qed.
+
+  Lemma preord_env_refl k :
+    Reflexive (preord_val k) ->
+    Reflexive (preord_env k).
+  Proof.
+    intros H r. intros; eexists; eauto.
+  Qed.
+
+  Corollary preord_env_setlist_l (rho1 rho2 rho1' rho2' : env) (k : nat)
+        (xs : list var) (vs1 vs2 : list val) :
+    preord_env k rho1 rho2 ->
+    Forall2 (preord_val k) vs1 vs2 ->
+    setlist xs vs1 rho1 = Some rho1' ->
+    setlist xs vs2 rho2 = Some rho2' ->
+    preord_env k rho1' rho2'.
+  Proof.
+    intros. eapply preord_env_P_setlist_l; eauto.
+  Qed.
+
+  (** * Index Monotonicity Properties *)
+
+  (** The value relation is monotonic in the step index *)
+  Lemma preord_val_monotonic (k : nat) :
+    (forall v1 v2 j,
+       preord_val k v1 v2 -> j <= k -> preord_val j v1 v2).
+  Proof.
+    intros v1 v2 h Hpre Hleq. try rewrite preord_val_eq in *.
+    revert v2 Hpre; induction v1 using val_ind'; intros v2 Hpre;
+    destruct v2; try (simpl; contradiction); eauto.
+    - destruct l; try now inv Hpre.
+    - inv Hpre. inv H0.
+      split; auto. constructor; eauto; rewrite preord_val_eq in *.
+      eapply IHv1; eauto.
+      destruct (IHv0 ((Vconstr tau t1 l'))) as [Heq Hpre']; eauto.
+      simpl. split; eauto.
+    - intros vs1 vs2 j t1 xs e1 rho1' Hlen Hf Heq.
+      edestruct Hpre as [t2 [xs2 [e2 [rho2' [H1 [H2 H3]]]]]]; eauto.
+      do 4 eexists; split; eauto. split; eauto. intros Hleq' Hall. 
+      eapply H3; eauto. omega. 
+  Qed.
+  
+  (** The expression relation is monotonic in the step index *)
+  Lemma preord_exp_monotonic (k : nat) :
+    (forall rho1 e1 rho2 e2 j,
+       preord_exp k (rho1, e1) (rho2, e2) ->
+       j <= k -> preord_exp j (rho1, e1) (rho2, e2)).
+  Proof.
+    intros rho1 e1 rho2 e2 j Hpre Hleq v1 c1 Hlt Hstep.
+    edestruct (Hpre v1 c1) as [v2 [c2 [H1 H2]]]; eauto. omega.
+    do 2 eexists; split; eauto.
+    eapply preord_val_monotonic. eapply H2. omega.
+  Qed.
+
+  (** The environment relations are monotonic in the step index *)
+  Lemma preord_env_P_monotonic :
+    forall P (k j : nat) (rho1 rho2 : env),
+      j <= k -> preord_env_P P k rho1 rho2 -> preord_env_P P j rho1 rho2.
+  Proof.
+    intros P k j rho1 rho2 Hleq Hpre x HP v Hget.
+    edestruct Hpre as [v2 [Heq Hpre2]]; eauto.
+    eexists; split; eauto. eapply preord_val_monotonic; eauto.
+  Qed.
+  
+  Lemma preord_env_monotonic k j rho1 rho2 :
+    j <= k -> preord_env k rho1 rho2 -> preord_env j rho1 rho2.
+  Proof.
+    intros Hleq H. eapply preord_env_P_monotonic; eauto.
+  Qed.
+  
+  (** * Compatibility Properties *)
+
+  Lemma preord_exp_const_compat k rho1 rho2 x x' tau t ys1 ys2 e1 e2 :
+    Forall2 (preord_var_env k rho1 rho2) ys1 ys2 ->
+    (forall vs1 vs2 : list val,
+       Forall2 (preord_val k) vs1 vs2 ->
+       preord_exp k (e1, M.set x (Vconstr tau t vs1) rho1)
+                  (e2, M.set x' (Vconstr tau t vs2) rho2)) ->
+    preord_exp k (Econstr x tau t ys1 e1, rho1) (Econstr x' tau t ys2 e2, rho2).
+  Proof.
+    intros Hall Hpre v1 c1 Hleq1 Hstep1. inv Hstep1.
+    edestruct (preord_var_env_getlist rho1 rho2) as [vs2' [Hget' Hpre']];
+      [| eauto |]; eauto.
+    edestruct Hpre as [v2 [c2 [Hstep Hval]]]; eauto.
+    repeat eexists; eauto. econstructor; eauto.
+  Qed.
+
+  Lemma preord_exp_proj_compat k rho1 rho2 x x' tau n y1 y2 e1 e2 :
+    preord_var_env k rho1 rho2 y1 y2 ->
+    (forall v1 v2,
+       preord_val k v1 v2 -> 
+       preord_exp k (e1, M.set x v1 rho1)
+                  (e2, M.set x' v2 rho2)) ->
+    preord_exp k (Eproj x tau n y1 e1, rho1) (Eproj x' tau n y2 e2, rho2).
+  Proof.
+    intros Henv Hexp v1 c1 Hleq1 Hstep1. inv Hstep1.
+    edestruct Henv as [v' [Hget Hpre]]; eauto.
+    destruct v'; rewrite preord_val_eq in Hpre; simpl in Hpre; try contradiction.
+    inv Hpre.
+    edestruct (Forall2_asym_nthN (preord_val k) vs l) as [v2 [Hnth Hval]]; eauto.
+    edestruct Hexp as [v2' [c2 [Hstep Hval']]]; eauto.
+    repeat eexists; eauto. econstructor; eauto.
+  Qed.
+
+  Lemma Forall2_Forall2_asym_included {A} R (l1 l2 : list A) :
+    Forall2 R l1 l2 ->
+    Forall2_asym R l1 l2.
+  Proof.
+    intros H. induction H; eauto.
+  Qed.    
+  
+  Lemma preord_exp_app_compat k rho1 rho2 x1 x2 ys1 ys2 :
+    preord_var_env k rho1 rho2 x1 x2 ->
+    Forall2 (preord_var_env k rho1 rho2) ys1 ys2 ->
+    preord_exp k (Eapp x1 ys1, rho1) (Eapp x2 ys2, rho2).
+  Proof.
+    intros Hvar Hall v1 c1 Hleq1 Hstep1. inv Hstep1.
+    edestruct Hvar as [v2' [Hget Hpre]]; eauto.
+    rewrite preord_val_eq in Hpre.
+    destruct v2'; try (now simpl in Hpre; contradiction).
+    edestruct preord_var_env_getlist as [vs2 [Hget' Hpre']]; eauto.
+    edestruct (Hpre vs vs2 (k-1)) as [t2 [xs2 [e2 [rho2' [Hf [Hset H']]]]]]; eauto.
+    now eapply Forall2_length; eauto.
+    edestruct H' with (c1 := c) as [v2 [c2 [Hstep' Hpre'']]];
+      eauto; try omega.
+    - eapply Forall2_monotonic; [| now eauto ].
+        intros. eapply (preord_val_monotonic k); [ now eauto | omega ].
+    - repeat eexists. econstructor 4; eauto.
+      replace (k - (c + 1)) with (k - 1 - c) by omega. eauto.
+  Qed.
+
+  Lemma preord_exp_case_nil_compat k rho1 rho2 x1 x2 :
+    preord_exp k (Ecase x1 [], rho1) (Ecase x2 [], rho2).
+  Proof.
+    intros v1 c1 Hleq1 Hstep1. inv Hstep1. inv H3.
+  Qed.
+
+  Lemma preord_exp_case_cons_compat k rho1 rho2 x1 x2 c e1 e2 P1 P2:
+    preord_var_env k rho1 rho2 x1 x2 ->
+    preord_exp k (e1, rho1) (e2, rho2) ->
+    preord_exp k (Ecase x1 P1, rho1)
+               (Ecase x2 P2, rho2) ->
+    preord_exp k (Ecase x1 ((c, e1) :: P1), rho1)
+               (Ecase x2 ((c, e2) :: P2), rho2).
+  Proof.
+    intros Henv Hexp_hd Hexp_tl v1 c1 Hleq1 Hstep1. inv Hstep1. inv H3.
+    destruct (M.elt_eq c t) eqn:Heq; subst.
+    - inv H0. edestruct Hexp_hd as [v2 [c2 [Hstep2 Hpre2]]]; eauto.
+      edestruct Henv as [v2' [Hget Hpre]]; eauto.
+      rewrite preord_val_eq in Hpre.
+      destruct v2'; try (now simpl in Hpre; contradiction). inv Hpre. 
+      repeat eexists; eauto. econstructor; eauto. simpl; rewrite Heq; eauto.
+    - edestruct Hexp_tl as [v2 [c2 [Hstep2 Hpre2]]]; eauto.
+      econstructor; eauto. inv Hstep2.
+      edestruct Henv as [v2' [Hget Hpre]]; eauto.
+      rewrite preord_val_eq in Hpre.
+      destruct v2'; try (now simpl in Hpre; contradiction). inv Hpre.
+      rewrite Hget in H3; inv H3.
+      repeat eexists; eauto. econstructor; eauto. simpl; rewrite Heq; eauto.
+  Qed.
+  
+  Axiom Prim_axiom :
+    forall f f' v1,
+      M.get f pr = Some f' ->
+      forall k vs1 vs2,
+        Forall2 (preord_val k) vs1 vs2 ->
+        f' vs1 = Some v1 ->
+        exists v2,
+          f' vs2 = Some v2 /\                      
+          preord_val k v1 v2.
+  
+  Lemma preord_exp_prim_compat k rho1 rho2 x1 x2 tau f ys1 ys2 e1 e2 :
+    Forall2 (preord_var_env k rho1 rho2) ys1 ys2 ->
+    (forall v1 v2,
+       preord_val k v1 v2 -> 
+       preord_exp k (e1, M.set x1 v1 rho1)
+                  (e2, M.set x2 v2 rho2)) ->
+    preord_exp k (Eprim x1 tau f ys1 e1, rho1) (Eprim x2 tau f ys2 e2, rho2).
+  Proof.
+    intros Henv Hexp v1 c1 Hleq1 Hstep1. inv Hstep1.
+    edestruct preord_var_env_getlist as [vs2 [Hget' Hpre']]; eauto.
+    edestruct Prim_axiom as [v2 [Heq Hprev2]]; eauto.
+    edestruct Hexp as [v2' [c2 [Hstepv2' Hprev2']]]; eauto.
+    repeat eexists; eauto. econstructor; eauto.
+  Qed.
+
+  Lemma preord_exp_fun_compat k rho1 rho2 B B' e1 e2 :
+    preord_exp k (e1, def_funs B B rho1 rho1)
+               (e2, def_funs B' B' rho2 rho2) ->
+    preord_exp k (Efun B e1, rho1) (Efun B' e2, rho2).
+  Proof.
+    intros Hexp v1 c1 Hleq1 Hstep1. inv Hstep1.
+    edestruct Hexp as [v2' [c2 [Hstepv2' Hprev2']]]; eauto.
+    repeat eexists; eauto. econstructor; eauto.
+  Qed.
+
+
+  (** * Reflexivity Properties *)
+
+  (** Un-nesting the function case of the reflexivity proof *)
+  Lemma preord_env_P_def_funs_pre k B rho rho' B' e :
+    (* The inductive hypothesis on expressions *)
+    (forall m e (rho rho' : env),
+       m <  k ->
+       preord_env_P (fun x => occurs_free e x) m rho rho' ->
+       preord_exp m (e, rho) (e, rho')) ->
+    (* Environments are related at FV(Efun B' e) *) 
+    preord_env_P (occurs_free (Efun B' e)) k rho rho' ->
+    preord_env_P (Union _ (occurs_free (Efun B' e)) (name_in_fundefs B))
+                 k (def_funs B' B rho rho) (def_funs B' B rho' rho').
+   Proof.
+    revert B rho rho' e B'.
+    induction k as [ k IH' ] using lt_wf_rec1. intros B rho rho' e B'.
+    induction B; intros Hyp Hpre.
+    - simpl. apply preord_env_P_extend.
+      + eapply preord_env_P_antimon; [ now eapply IHB; eauto | ].
+        rewrite !Setminus_Union_distr, Setminus_Empty_set, Union_Empty_set_r.
+        eapply Included_Union_compat.
+        * eapply Setminus_Included. now apply Included_refl.
+        * eapply Subset_Setminus.
+      + rewrite preord_val_eq.
+        intros vs1 vs2 j t1 xs1 e1 rho1' Hlen Hf Hs.
+        edestruct setlist_length as [rho2' Hs']; eauto.
+        exists t1. exists xs1. exists e1. exists rho2'. split; eauto.
+        split; [ now eauto |]. intros Hleq Hpre'. 
+        eapply Hyp. omega.
+        eapply preord_env_P_setlist_l; [| | eauto | eauto | eauto]. 
+        * apply IH'; eauto. intros. apply Hyp. omega. eauto.
+          eapply (preord_env_P_monotonic _ k); eauto. omega.
+        * intros x Hin Hfr. simpl.
+          apply find_def_correct in Hf; eauto.
+          specialize (occurs_free_in_fun _ _ _ _ _ Hf x Hfr); intros H1.
+          inv H1; eauto; try contradiction. inv H.
+          now right; eauto. now left; eauto.
+    - simpl. intros x HP. inv HP. inv H. apply Hpre; eauto.
+      apply Hpre; eauto. inv H.
+   Qed.
+  
+  Lemma preord_exp_refl k e rho rho' :
+    preord_env_P (occurs_free e) k rho rho' ->
+    preord_exp k (e, rho) (e, rho').
+  Proof.
+    revert e rho rho'.
+    (* Well founded induction on the step-index *)
+    induction k as [ k IH ] using lt_wf_rec1.
+    (* Induction on e *)
+    induction e using exp_ind'; intros rho rho' Henv.
+    (* Each case follows from the corresponding compat lemma *)
+    - eapply preord_exp_const_compat; eauto; intros.
+      * eapply Forall2_same. intros x HIn. apply Henv. now constructor.
+      * eapply IHe. eapply preord_env_P_extend.
+        eapply preord_env_P_antimon; eauto. intros x [H1 H2].
+        constructor 2; eauto. intros Hc. subst. now eauto.
+        rewrite preord_val_eq. constructor; eauto using Forall2_Forall2_asym_included.
+    - eapply preord_exp_case_nil_compat.
+    - eapply preord_exp_case_cons_compat; eauto.
+      apply IHe. intros x P. apply Henv. constructor; eauto.
+      apply IHe0. intros x P. apply Henv. apply Free_Ecase3; eauto.
+    - eapply preord_exp_proj_compat; eauto.
+      intros v1 v2 Hval. eapply IHe. eapply preord_env_P_extend; eauto.
+      eapply preord_env_P_antimon; eauto.
+      intros x [H1 H2]. constructor; eauto. intros Hc; subst; eauto.
+    - eapply preord_exp_fun_compat; eauto.
+      eapply IHe. eapply preord_env_P_antimon. 
+      now eapply preord_env_P_def_funs_pre; eauto.
+      now eapply occurs_free_Efun_Included.
+    - eapply preord_exp_app_compat.
+      intros x HP. apply Henv; eauto.
+      apply Forall2_same. intros. apply Henv. now constructor.
+    - eapply preord_exp_prim_compat; eauto; intros.
+      eapply Forall2_same. intros. apply Henv. now constructor.
+      eapply IHe. eapply preord_env_P_extend; eauto.
+      eapply preord_env_P_antimon; eauto. intros x [H1 H2].
+      apply Free_Eprim2; eauto. intros Hc; subst; eauto.
+  Qed.
+  (* Note: I think that the above proof could go through also by mutual
+     induction on expressions and function definitions and then nested induction
+     at the step-index only for the function case *)
+
+  Lemma preord_env_P_def_funs k B rho rho' B' S1 :
+    preord_env_P (fun x => (~ name_in_fundefs B' x /\ S1 x) \/
+                        occurs_free_fundefs B' x) k rho rho' ->
+    preord_env_P (fun x => (~ name_in_fundefs B' x /\ S1 x) \/
+                           occurs_free_fundefs B' x \/ name_in_fundefs B x)
+                 k (def_funs B' B rho rho) (def_funs B' B rho' rho').
+  Proof.
+    intros Hpre.
+    revert B rho rho' B' Hpre.
+    induction k as [ k IH' ] using lt_wf_rec1. intros B rho rho' B' Hpre.
+    induction B.
+    - simpl. apply preord_env_P_extend.
+      + intros x H. inv H. eapply IHB; eauto.
+        inv H0; eauto. inv H; eauto. inv H0; try contradiction; eauto.
+      + rewrite preord_val_eq.
+        intros vs1 vs2 j t1 xs1 e1 rho1' Hlen Hf Hs.
+        edestruct setlist_length as [rho2' Hs']; eauto.
+        exists t1. exists xs1. exists e1. exists rho2'. split; eauto.
+        split. eauto. intros Hleq Hpre'.
+        eapply preord_exp_refl. 
+        eapply preord_env_P_setlist_l; [| | eauto | eauto | eauto].
+        apply IH'; eauto. 
+        eapply (preord_env_P_monotonic _ k); eauto. omega.
+        intros x Hin Hfr. 
+        apply find_def_correct in Hf.
+        edestruct (occurs_free_in_fun _ _ _ _ _ Hf x Hfr); eauto; try contradiction.
+        inv H; eauto.
+    - simpl. intros x HP. inv HP. apply Hpre; eauto. inv H.
+      apply Hpre; eauto. inv H0.
+  Qed.
+
+  Corollary preord_env_P_def_funs_col k B rho rho' S1 :
+    preord_env_P (Union var (Setminus var S1 (name_in_fundefs B))
+                        (occurs_free_fundefs B)) k rho rho' ->
+    preord_env_P S1 k (def_funs B B rho rho) (def_funs B B rho' rho').
+  Proof.
+    intros Hpre. eapply preord_env_P_antimon.
+    - eapply preord_env_P_def_funs; eauto.
+      eapply preord_env_P_antimon; eauto.
+      intros x HS. inv HS. inv H. left. constructor; eauto.
+      right; eauto.
+    - intros x HS.
+      destruct (@Dec _ _ (Decidable_name_in_fundefs B) x); eauto.
+  Qed.
+  
+  Lemma preord_exp_refl_weak (k : nat) e rho rho' :
+      preord_env k rho rho' ->
+      preord_exp k (e, rho) (e, rho').
+  Proof.
+    intros Henv. eapply preord_exp_refl.
+    eapply preord_env_P_antimon; eauto.
+    intros x H; simpl; eauto.
+  Qed.
+  
+  Lemma preord_val_refl (k : nat) :
+    Reflexive (preord_val k).
+  Proof.
+    induction k using lt_wf_rec1.
+    destruct k as [| k]; unfold Reflexive; intros x; rewrite preord_val_eq;
+    induction x using val_ind'; simpl; eauto;
+    try (now (try split; eauto); econstructor; eauto; rewrite preord_val_eq; eauto).
+    - split; eauto. constructor; eauto. rewrite preord_val_eq; eauto.
+      destruct IHx0. eauto.
+    - intros.
+      edestruct (setlist_length (def_funs f0 f0 t t) (def_funs f0 f0 t t))
+        as [rho2' Hset']; eauto.
+      do 4 eexists; split; eauto. split; eauto. intros Hc.
+      exfalso. omega.
+    - split; eauto. constructor; eauto. rewrite preord_val_eq; eauto.
+        destruct IHx0. eauto.
+    - intros.
+      edestruct (setlist_length (def_funs f0 f0 t t) (def_funs f0 f0 t t))
+        as [rho2' Hset']; eauto.
+      do 4 eexists; eauto. split; eauto. split; eauto.
+      intros Hleq Hall v1 c Hleq' Hstep. 
+      eapply preord_exp_refl_weak; eauto.
+      eapply preord_env_setlist_l; eauto.
+      eapply preord_env_refl; eauto.
+  Qed.
+
+  Lemma preord_env_P_refl S k rho :
+    preord_env_P S k rho rho.
+  Proof.
+    intros x Px v Hget.
+    eexists; split; eauto. eapply preord_val_refl; eauto.
+  Qed.
+
+  Lemma preord_env_def_funs k f rho1 rho2 :
+    preord_env k rho1 rho2 ->
+    preord_env k (def_funs f f rho1 rho1) (def_funs f f rho2 rho2).
+  Proof.
+    intros Henv. eapply preord_env_P_def_funs_col.
+    eapply preord_env_P_antimon; eauto. intros x H; simpl; eauto.
+  Qed.
+
+  Lemma preord_exp_case_compat k rho1 rho2 x c e1 e2 P1' P1 :
+    preord_env_P (occurs_free (Ecase x (P1' ++ ((c, e1) :: P1)))) k rho1 rho2 ->
+    preord_exp k (e1, rho1) (e2, rho2) ->
+    preord_exp k (Ecase x (P1' ++ ((c, e1) :: P1)), rho1)
+               (Ecase x (P1' ++ ((c, e2) :: P1)), rho2).
+  Proof.
+    (* TODO : this lemma could be used to refactor hoisting correctness proof *)
+    induction P1' as [| [c' e'] P1' IHP1']; simpl;
+    intros Henv Hexp v1 c1 Hleq1 Hstep1.
+    - inv Hstep1. simpl in H3. edestruct Henv as [v2' [Hget Hpre]]; eauto.
+      rewrite preord_val_eq in Hpre.
+      destruct v2'; try (now simpl in Hpre; contradiction). inv Hpre.
+      destruct (M.elt_eq c t1) eqn:Heq; subst.
+      + inv H3. edestruct Hexp as [v2 [c2 [Hstep2 Hpre2]]]; eauto.
+        repeat eexists; eauto. econstructor; eauto. simpl; rewrite Heq; eauto.
+      + edestruct (preord_exp_refl k e) as [v2 [c2 [Hstep2 Hpre2]]]; eauto.
+        * eapply preord_env_P_antimon; [ eassumption | ].
+          intros x' H'. eapply occurs_free_Ecase_Included; eauto.
+          right. eapply findtag_In_patterns; eauto.
+        * repeat eexists; eauto. econstructor; eauto. simpl; rewrite Heq; eauto.
+    - inv Hstep1. simpl in H3. edestruct Henv as [v2' [Hget Hpre]]; eauto.
+      rewrite preord_val_eq in Hpre.
+      destruct v2'; try (now simpl in Hpre; contradiction). inv Hpre.
+      destruct (M.elt_eq c' t1) eqn:Heq; subst.
+      + inv H3.
+        edestruct (preord_exp_refl k e) as [v2 [c2 [Hstep2 Hpre2]]]; eauto.
+        *eapply preord_env_P_antimon; [ eassumption | ].
+          intros x' H'. eapply occurs_free_Ecase_Included; eauto. now left. 
+        * repeat eexists; eauto. econstructor; eauto. simpl; rewrite Heq; eauto.
+      + edestruct IHP1' as [v2 [c2 [Hstep2 Hpre2]]]; eauto; eauto.
+        * eapply preord_env_P_antimon; [ eassumption | ].
+          intros x' H'. eapply Free_Ecase3; eauto. 
+        * econstructor; eauto.
+        * inv Hstep2. rewrite Hget in H4; inv H4.
+          repeat eexists; eauto. econstructor; eauto. simpl. rewrite Heq; eauto.
+  Qed.
+
+  (* TODO : move *)
+  Lemma find_def_def_funs_ctx B f e1 e2 tau xs e' :
+    find_def f (B <[ e1 ]>) = Some (tau, xs, e') ->
+    (find_def f (B <[ e2 ]>) = Some (tau, xs, e')) \/
+    (exists c, e' = c |[ e1 ]| /\
+              find_def f (B <[ e2 ]>) = Some (tau, xs, c |[ e2 ]|)).
+  Proof.
+    revert tau xs e'. induction B; simpl; intros tau xs e' Heq.
+    - destruct (M.elt_eq f v).
+      + inv Heq. right. eexists e.
+        split; eauto.
+      + left; eauto.
+    - destruct (M.elt_eq f v).
+      + inv Heq. left; eauto.
+      + eauto.
+  Qed.
+
+  (** * Compatibility with context application *)
+
+  Lemma preord_env_P_def_funs_compat_pre k B rho1 rho2 B' e1 e2 S1 :
+    (forall m c (rho1 rho2 : env),
+       m <  k ->
+       preord_env_P (occurs_free (c |[ e1 ]|)) m rho1 rho2 ->
+       preord_exp m (c |[ e1 ]|, rho1) (c |[ e2 ]|, rho2)) ->
+    preord_env_P (Union _ (occurs_free_fundefs (B' <[ e1 ]>))
+                        (Setminus _ S1 (name_in_fundefs (B' <[ e1 ]>))))
+                 k rho1 rho2 ->
+    preord_env_P (Union _ (Setminus _ S1 (name_in_fundefs (B' <[ e1 ]>)))
+                        (Union _ (occurs_free_fundefs (B' <[ e1 ]>))
+                               (name_in_fundefs (B <[ e1 ]>))))
+                 k (def_funs (B' <[ e1 ]>) (B <[ e1 ]>) rho1 rho1)
+                 (def_funs (B' <[ e2 ]>) (B <[ e2 ]>) rho2 rho2).
+  Proof.
+    revert B rho1 rho2 B' e1 e2 S1.
+    induction k as [ k IH' ] using lt_wf_rec1.
+    intros B rho1 rho2 B' e1 e2 S1 Hpre Henv.
+    assert (Hval : forall f, preord_val k (Vfun rho1 (B' <[ e1 ]>) f)
+                                   (Vfun rho2 (B' <[ e2 ]>) f)).
+    { intros f. rewrite preord_val_eq.
+      intros vs1 vs2 j t1 xs1 e' rho1' Hlen Hf Hs.
+      edestruct find_def_def_funs_ctx as [H1 | [c [H1 H2]]]; eauto.
+      + edestruct setlist_length as [rho2' Hs']; eauto.
+        do 5 eexists; eauto. split; eauto.
+        intros Hleq Hall.
+        eapply preord_exp_refl.
+        eapply preord_env_P_setlist_l; [| | eauto | eauto | eauto ].
+        eapply IH'; eauto. 
+        intros. eapply Hpre; eauto. omega. 
+        eapply preord_env_P_monotonic; [| eassumption ]. omega.
+        intros x H Hfv. 
+        eapply find_def_correct in Hf; eauto.
+        eapply occurs_free_in_fun in Hfv; eauto.
+        inv Hfv. exfalso. eauto. right. eapply Union_sym. eauto.
+      + subst. edestruct setlist_length as [rho2' Hs']; eauto.
+        do 5 eexists; eauto. split; eauto.
+        intros Hleq Hall. eapply Hpre; eauto.
+        eapply preord_env_P_setlist_l; [| | eauto | eauto | eauto ].
+        eapply IH'; eauto.
+        intros. eapply Hpre; eauto. omega. 
+        eapply preord_env_P_monotonic; [| eassumption ]. omega.
+        intros x H Hfv. 
+        eapply find_def_correct in Hf; eauto.
+        eapply occurs_free_in_fun in Hfv; eauto.
+        inv Hfv. exfalso. eauto. right. eapply Union_sym. eauto. }
+    induction B.
+    - simpl. apply preord_env_P_extend.
+      + induction f.
+        { simpl. apply preord_env_P_extend.
+          - eapply preord_env_P_antimon; [ eassumption |]. 
+            rewrite !Setminus_Union_distr.
+            repeat rewrite Setminus_Empty_set at 1. rewrite !Union_Empty_set_r.
+            rewrite (Setminus_Included_Empty_set (Empty_set var) (Singleton var v0));
+              [| intros x' H'; now inv H' ].
+            rewrite Union_Empty_set_r.
+            rewrite (Setminus_Included_Empty_set
+                       (Setminus var (Singleton var v0) (Singleton var v)));
+              [| eapply Setminus_Included; now apply Included_refl ].
+            rewrite Union_Empty_set_r.
+            rewrite <- Setminus_Union_distr.
+            eapply Included_Union_compat;
+              eapply Setminus_Included; now apply Included_refl.
+          - eapply Hval. }
+        { simpl. eapply preord_env_P_antimon ; [ eassumption |].
+          rewrite Setminus_Union_distr, Union_Empty_set_l.
+          rewrite Setminus_Union_Inlcluded; eauto using Included_refl.
+          rewrite <- Setminus_Union_distr, Union_sym.
+          apply Setminus_Included; eauto using Included_refl. }
+      + eapply Hval.
+    - simpl. apply preord_env_P_extend.
+      + eapply preord_env_P_antimon; [now eauto |].
+        rewrite !Setminus_Union_distr, Setminus_Empty_set, Union_Empty_set_r.
+        rewrite <- !Setminus_Union_distr.  
+        apply Setminus_Included; eauto using Included_refl.
+      + apply Hval.
+  Qed.
+  
+  Lemma preord_exp_compat k rho1 rho2 c e1 e2 :
+    (forall k rho1 rho2, preord_env_P (occurs_free e1) k rho1 rho2 ->
+                    preord_exp k (e1, rho1) (e2, rho2)) ->
+    preord_env_P (occurs_free (c |[ e1 ]|)) k rho1 rho2 ->
+    preord_exp k (c |[ e1 ]|, rho1) (c |[ e2 ]|, rho2).
+  Proof.
+    revert c rho1 rho2 e1 e2. induction k as [ k IH' ] using lt_wf_rec1.
+    induction c; intros rho1 rho2 e1 e2 Hyp Hpre; eauto.
+    - simpl. eapply preord_exp_const_compat; eauto.
+      + eapply Forall2_same. intros x Hin. eapply Hpre. constructor; eauto.
+      + intros vs1 vs2 Hall. eapply IHc; eauto.
+        eapply preord_env_P_extend.
+        * eapply preord_env_P_antimon; eauto.
+          simpl. intros x H. inv H. constructor 2; eauto.
+          intros H. subst; eauto.
+        * rewrite preord_val_eq. simpl; split; eauto using Forall2_Forall2_asym_included.
+    - simpl. eapply preord_exp_proj_compat; eauto.
+      + eapply Hpre. constructor; eauto.
+      + intros vs1 vs2 Hall. eapply IHc; eauto.
+        eapply preord_env_P_extend; [| assumption ].
+        eapply preord_env_P_antimon; eauto.
+        simpl. intros x H. inv H. constructor; eauto.
+        intros H. subst; eauto.
+    - simpl. eapply preord_exp_prim_compat; eauto.
+      + eapply Forall2_same. intros x Hin. eapply Hpre. constructor; eauto.
+      + intros vs1 vs2 Hall. eapply IHc; eauto.
+        eapply preord_env_P_extend; [| assumption ].
+        eapply preord_env_P_antimon; eauto.
+        simpl. intros x H. inv H. eapply Free_Eprim2; eauto.
+        intros H. subst; eauto.
+    - simpl. eapply preord_exp_case_compat; eauto.
+      eapply IHc; auto. eapply preord_env_P_antimon; eauto.
+      simpl. intros x H.
+      eapply occurs_free_Ecase_Included; eauto.
+      eapply in_or_app. right. left; eauto.
+    - simpl. eapply preord_exp_fun_compat; eauto.
+      eapply IHc; auto.
+      eapply preord_env_P_def_funs_col.
+      eapply preord_env_P_antimon; [ eassumption |].
+      intros x' H'. inv H'.
+      + inv H. simpl. constructor; eauto.
+      + simpl. eapply Free_Efun2; eauto.
+    - intros v1 c1 Hleq Hstep. inv Hstep.
+      edestruct (preord_exp_refl k e) as [v2 [c2 [Hstep1 Henv2]]]; eauto.
+      + eapply preord_env_P_antimon.
+        * eapply preord_env_P_def_funs_compat_pre; eauto.
+          eapply preord_env_P_antimon; [ eassumption |].
+          intros x' H'. simpl. inv H'.
+          now eapply Free_Efun2.
+          inv H. constructor; eauto.
+        * eapply Included_trans.
+          eapply occurs_free_Efun_Included. intros x H.
+          inv H. inv H0; eauto. left; constructor; eauto.
+          right. right; eauto.
+      + repeat eexists; eauto. simpl. constructor; eauto.
+  Qed.
+
+  (** * Transitivity Properties *)
+
+  (** Expression relation is transitive *)
+  Lemma preord_exp_trans_pre (k : nat) :
+    (* The induction hypothesis for transitivity of
+       the value relation. They need to be proved simultaneously *)
+    (forall k' v1 v2 v3,
+       k' <= k ->
+       preord_val k' v1 v2 ->
+       (forall m, preord_val m v2 v3) ->
+       preord_val k' v1 v3) ->
+    forall rho1 rho2 rho3 e1 e2 e3,
+      preord_exp k (e1, rho1) (e2, rho2) ->
+      (forall m, preord_exp m (e2, rho2) (e3, rho3)) ->
+      preord_exp k (e1, rho1) (e3, rho3).
+  Proof.
+    intros Htrans rho1 rho2 rho3 e1 e2 e3 H1 H2 v1 c1 Hleq1 Hstep1.
+    edestruct H1 as [v2 [c2 [Hstep2 Hpre2]]]; eauto. 
+    edestruct (H2 c2) as [v3 [c3 [Hstep3 Hpre3]]]; [| eauto |]. omega.
+    exists v3, c3. split; eauto.
+    eapply Htrans. omega. eauto. intros m.
+    edestruct (H2 (m + c2)) as [v3' [c3' [Hstep3' Hpre3']]]; [| eauto |]. omega.
+    eapply bstep_e_deterministic in Hstep3; eauto. inv Hstep3.
+    eapply preord_val_monotonic; eauto. omega.
+  Qed.
+
+  Lemma preord_val_trans (k : nat) v1 v2 v3 :
+    preord_val k v1 v2 ->
+    (forall m, preord_val m v2 v3) ->
+    preord_val k v1 v3.
+  Proof.
+    revert v1 v2 v3.
+    induction k using lt_wf_rec1.
+    intros x; induction x using val_ind'; simpl; eauto;
+    intros v1 v2;
+    try (now  intros H1 H2; specialize (H2 k); rewrite !preord_val_eq in *;
+           destruct v1; destruct v2; 
+         try (now simpl in *; contradiction); inv H1; inv H2; simpl; eauto).
+    - intros H1 H2. assert (H2' := H2 k); rewrite !preord_val_eq in *.
+      destruct v1; destruct v2; try (now simpl in *; contradiction).
+      destruct H1 as [H1 H1']. destruct H2' as [H3 H3']. subst.
+      destruct l0; try inv H1'; try inv H3'. split; eauto. 
+      econstructor; eauto.
+      + eapply IHx. eassumption.
+        intros m. specialize (H2 m). rewrite !preord_val_eq in H2.
+        inv H2. now inv H1.
+      + assert
+          (Hsuf :
+             preord_val k (Vconstr tau t3 l) (Vconstr tau t3 l')).
+        { eapply IHx0 with (v2 := Vconstr tau t3 l0); [| intros m];
+          rewrite !preord_val_eq in *. simpl. split; eauto.
+          specialize (H2 m). rewrite !preord_val_eq in H2.
+          split; eauto. inv H2. now inv H1. }
+        rewrite !preord_val_eq in Hsuf. now inv Hsuf.
+    - intros H1 H2. assert (H2' := H2 k); rewrite !preord_val_eq in *.
+      destruct v1; destruct v2; try (now simpl in *; contradiction).
+      intros vs1 vs3 j t1' xs1 e1 rho1' Hlen Hf Hs.
+      edestruct (H1 vs1 vs3) as [t2' [xs2 [e2 [rho2 [Hf2 [Hs2 Hpre2]]]]]]; eauto.
+      edestruct (H2' vs3 vs3) with (j := 0) as [t3' [xs3 [e3 [rho3 [Hf3 [Hs3 Hpre3]]]]]]; eauto.
+      do 4 eexists; split; eauto. split; eauto. intros Hlt Hall.
+      eapply preord_exp_trans_pre. intros. eapply H; eauto. omega.
+      eapply Hpre2; eauto.
+      intros m. specialize (H2 (m + 1)). rewrite !preord_val_eq in H2.
+      edestruct (H2 vs3 vs3) with (j := m)
+        as [t3'' [xs3' [e3' [rho3' [Hf3' [Hs3' Hpre3']]]]]]; eauto.
+      rewrite Hf3 in Hf3'. inv Hf3'. rewrite <- Hs3 in Hs3'. inv Hs3'.
+      eapply Hpre3'; eauto. omega. eapply Forall2_refl. now eapply preord_val_refl.
+  Qed.
+
+  Lemma preord_env_P_trans (k : nat) P rho1 rho2 rho3 :
+    preord_env_P P k rho1 rho2 ->
+    (forall m,  preord_env_P P m rho2 rho3) ->
+    preord_env_P P k rho1 rho3.
+  Proof.
+    intros H1 H2 x Px v Hget. assert (H2' := (H2 k)).
+    edestruct H1 as [v' [Hget' Hpre']]; eauto.
+    edestruct H2' as [v'' [Hget'' Hpre'']]; eauto.
+    eexists; split; eauto. eapply preord_val_trans; eauto.
+    intros m.
+    edestruct (H2 m) as [v''' [Hget''' Hpre''']]; eauto.
+    rewrite Hget'' in Hget'''. now inv Hget'''.
+  Qed.
+  
+  Corollary preord_exp_trans (k : nat) :
+    forall rho1 rho2 rho3 e1 e2 e3,
+      preord_exp k (e1, rho1) (e2, rho2) ->
+      (forall m, preord_exp m (e2, rho2) (e3, rho3)) ->
+      preord_exp k (e1, rho1) (e3, rho3).
+  Proof.
+    intros. eapply preord_exp_trans_pre; eauto.
+    intros. eapply preord_val_trans; eauto.
+  Qed.
+
+  Lemma preord_env_P_def_funs_pre' k (P1 P2 : var -> Prop) B rho1 rho2 :
+    preord_env_P P1 k rho1 rho2 ->
+    (forall x, P2 x -> P1 x) -> 
+    (forall m (rho rho' : env) (e : exp),
+       m <  k ->
+       preord_env_P P1 m rho rho' ->
+       preord_exp m (e, rho) (e, rho')) ->
+    preord_env_P P2 k (def_funs B B rho1 rho1) (def_funs B B rho2 rho2).
+  Proof.
+    generalize B at 1 3. revert P1 P2 B rho1 rho2.
+    induction k as [ k IH' ] using lt_wf_rec1. intros P1 P2 B.
+    induction B; intros rho rho2 B' Henv Hyp1 Hyp2 x HP.
+    - simpl. apply preord_var_env_extend; eauto.
+      + eapply IHB; eauto.
+      + rewrite preord_val_eq.
+        intros vs1 vs2 j t1 xs1 e1 rho1' Hlen Hf Hs.
+        edestruct setlist_length as [rho2' Hs']; eauto.
+        exists t1. exists xs1. exists e1. exists rho2'. split; eauto.
+        split. eauto. intros Hleq Hpre. 
+        eapply Hyp2; try omega.
+        eapply preord_env_P_setlist_l; eauto.
+        eapply IH'; try omega; eauto. 
+        eapply preord_env_P_monotonic; [| eauto]. omega.
+        intros. eapply Hyp2; eauto. omega.
+    - simpl. eauto.
+  Qed.
+
+  (* TODO fix typo *)
+  Lemma preord_exp_proord_env_com rho1 rho2 rho1' rho2' e1 e2 :
+    (forall k, preord_exp k (e1, rho1) (e2, rho2)) ->
+    (forall k, preord_env_P (occurs_free e1) k rho1' rho1) ->
+    (forall k, preord_env_P (occurs_free e2) k rho2 rho2') ->
+    (forall k, preord_exp k (e1, rho1') (e2, rho2')).
+  Proof.
+    intros Hexp1 Henv1 Henv2 k.
+    eapply preord_exp_trans.
+    - now eapply preord_exp_refl.
+    - intros m. eapply preord_exp_trans; [ now eauto | ].
+      intros m'. now eapply preord_exp_refl.
+  Qed.
+
+  Lemma preord_env_permut k x y v1 v2 rho1 rho2 P :
+    x <> y ->
+    preord_env_P k P (M.set x v1 (M.set y v2 rho1)) (M.set x v1 (M.set y v2 rho2)) ->
+    preord_env_P k P (M.set x v1 (M.set y v2 rho1)) (M.set y v2 (M.set x v1 rho2)).
+  Proof.
+    intros Hneq Hpre x' HP v1' Hget.
+    rewrite M.gsspec in Hget.
+    destruct (Coqlib.peq x' x). inv Hget. 
+    - edestruct (Hpre x) as [v1'' [Hget'' Hpre'']]; eauto. rewrite M.gss; eauto.
+      rewrite M.gss in Hget''; inv Hget''.
+      eexists. rewrite M.gso; eauto. rewrite M.gss; eauto.
+    - edestruct (Hpre x') as [v1'' [Hget'' Hpre'']]; eauto.
+      rewrite M.gso; eauto. rewrite M.gsspec in Hget.
+      destruct (Coqlib.peq x' y). inv Hget.
+      + eexists. rewrite M.gss; eauto. split; eauto.
+        eapply preord_val_refl.
+      + do 2 (rewrite M.gso in Hget''; eauto).
+        eexists. split; eauto.
+        do 2 (rewrite M.gso; eauto).
+  Qed.
+
+  (** Left weakening *)
+  Lemma preord_env_P_set_not_in_P_l x v P k rho1 rho2 :
+    preord_env_P P k rho1 rho2 ->
+    Disjoint var P (Singleton var x) ->
+    preord_env_P P k (M.set x v rho1) rho2.
+  Proof.
+    intros Hpre HP x' HP' v' Hget.
+    rewrite M.gsspec in Hget. destruct (Coqlib.peq x' x).
+    - inv Hget. exfalso. inv HP. eapply H; eauto.
+    - edestruct Hpre; eauto.
+  Qed.
+
+  (** Right weakening *)
+  Lemma preord_env_P_set_not_in_P_r x v P k rho1 rho2 :
+    preord_env_P P k rho1 rho2 ->
+    Disjoint var P (Singleton var x) ->
+    preord_env_P P k rho1 (M.set x v rho2).
+  Proof.
+    intros Hpre HP x' HP' v' Hget.
+    rewrite M.gsspec. destruct (Coqlib.peq x' x); subst.
+    - exfalso; eauto. inv HP. eapply H; eauto.
+    - edestruct Hpre; eauto.
+  Qed.
+
+  (** Left weakening for function definitions *)
+  Lemma preord_env_P_def_funs_not_in_P_l B B' P k rho rho1 rho2 :
+    preord_env_P P k rho1 rho2 ->
+    Disjoint var P (name_in_fundefs B) ->
+    preord_env_P P k (def_funs B' B rho rho1) rho2.
+  Proof.
+    intros Hpre HP x' HP' v' Hget.
+    eapply def_funs_spec in Hget.
+    destruct Hget as [[Hname Heq] | [Hname Heq ]]; subst.
+    - exfalso. eapply HP; eauto.
+    - edestruct Hpre; eauto.
+  Qed.
+
+  (** Right weakening for function definitions *)
+  Lemma preord_env_P_def_funs_not_in_P_r B B' P k rho rho1 rho2 :
+    preord_env_P P k rho1 rho2 ->
+    Disjoint var P (name_in_fundefs B) ->
+    preord_env_P P k rho1 (def_funs B' B rho rho2).
+  Proof.
+    intros Hpre HP x' HP' v' Hget.
+    edestruct (@Dec _ _ (Decidable_name_in_fundefs B) x').
+    - exfalso. eapply HP; eauto.
+    - edestruct Hpre as [v'' [Hget' Hpre']]; eauto.
+      eexists. rewrite def_funs_neq; eauto.
+  Qed.
+
+  (** Left weakening for setlist *)
+  Lemma preord_env_P_setlist_not_in_P_r xs vs P k rho1 rho2 rho2' :
+    preord_env_P P k rho1 rho2 ->
+    Some rho2' = setlist xs vs rho2 -> 
+    Disjoint var P (FromList xs) ->
+    preord_env_P P k rho1 rho2'.
+  Proof.
+    revert vs rho2'. induction xs; intros vs rho2' Hpre Hset HD.
+    - destruct vs; try discriminate. inv Hset; eauto.
+    - destruct vs; try discriminate. simpl in Hset.
+      destruct (setlist xs vs rho2) eqn:Heq ; try discriminate. inv Hset.
+      rewrite FromList_cons in HD. eapply Disjoint_sym in HD.
+      apply preord_env_P_set_not_in_P_r. eapply IHxs; eauto.
+      eapply Disjoint_sym. eapply Disjoint_Union_r; eauto.
+      eapply Disjoint_sym. eapply Disjoint_Union_l; eauto.
+  Qed.
+
+  (** Right weakening for setlist *)
+  Lemma preord_env_P_setlist_not_in_P_l xs vs P k rho1 rho2 rho1' :
+    preord_env_P P k rho1 rho2 ->
+    Some rho1' = setlist xs vs rho1 -> 
+    Disjoint var P (FromList xs) ->
+    preord_env_P P k rho1' rho2.
+  Proof.
+    revert vs rho1'. induction xs; intros vs rho1' Hpre Hset HD.
+    - destruct vs; try discriminate. inv Hset; eauto.
+    - destruct vs; try discriminate. simpl in Hset.
+      destruct (setlist xs vs rho1) eqn:Heq ; try discriminate. inv Hset.
+      rewrite FromList_cons in HD. eapply Disjoint_sym in HD.
+      apply preord_env_P_set_not_in_P_l. eapply IHxs; eauto.
+      eapply Disjoint_sym. eapply Disjoint_Union_r; eauto.
+      eapply Disjoint_sym. eapply Disjoint_Union_l; eauto.
+  Qed.
+
+  Lemma preord_env_P_singleton_extend (rho1 rho2 : env) (k : nat) (x : var)
+        (v1 v2 : val) :
+    preord_val k v1 v2 ->
+    preord_env_P (Singleton var x) k (M.set x v1 rho1) (M.set x v2 rho2).
+  Proof.
+    intros Hpre. eapply preord_env_P_extend; eauto.
+    eapply preord_env_P_antimon. apply preord_env_Empty_set.
+    intros x' H. inv H. inv H0. exfalso. eauto.
+  Qed.
+
+  (** * Technical lemmas about mutually recursive function definitions *)
+
+  Lemma preord_env_set_def_funs_permut k x S1 B v1 v2 rho1 rho2 :
+    ~ bound_var_fundefs B x ->
+    closed_fundefs B ->
+    preord_val k v1 v2 ->
+    preord_env_P S1 k rho1 rho2 ->
+    preord_env_P (Union var S1 (Union var (Singleton var x) (name_in_fundefs B))) k
+                 (def_funs B B (M.set x v1 rho1) (M.set x v1 rho1)) 
+                 (M.set x v2 (def_funs B B rho2 rho2)).
+  Proof.
+    intros Hb Hclo Hval Hpre. rewrite (@Union_Setminus _ _ _ _).
+    apply preord_env_P_union.
+    - apply preord_env_P_def_funs_not_in_P_l;
+      eauto using Disjoint_Setminus, Included_Union_r, Included_Union_l.
+      apply preord_env_P_set_not_in_P_l;
+        eauto using Disjoint_Setminus, Included_Union_r, Included_Union_l.
+      apply preord_env_P_set_not_in_P_r;
+        eauto using Disjoint_Setminus, Included_Union_r, Included_Union_l.
+      apply preord_env_P_def_funs_not_in_P_r;
+        eauto using Disjoint_Setminus, Included_Union_r, Included_Union_l.
+      eapply preord_env_P_antimon. eauto.
+      apply Subset_Setminus.
+    - apply preord_env_P_union.
+      + apply preord_env_P_def_funs_not_in_P_l.
+        eapply preord_env_P_singleton_extend; eauto.
+        apply Disjoint_sym.
+        apply Disjoint_Singleton. intros Hc; apply Hb.
+        now apply name_in_fundefs_bound_var_fundefs.
+      + apply preord_env_P_set_not_in_P_r.
+        eapply preord_env_P_def_funs_col.
+        eapply preord_env_P_antimon. apply preord_env_Empty_set.
+        intros x' HIn. inv HIn. exfalso. inv H. contradiction.
+        unfold closed_fundefs in Hclo. rewrite <- Hclo; eauto.
+        apply Disjoint_Singleton. intros Hc; apply Hb.
+        now apply name_in_fundefs_bound_var_fundefs.
+  Qed. 
+
+  Lemma preord_env_def_funs_permut (k : nat) S1 (B1 B2 : fundefs) (rho1 rho2 : env) :
+    closed_fundefs B1 -> closed_fundefs B2 ->
+    Disjoint var (name_in_fundefs B1) (name_in_fundefs B2) ->
+    preord_env_P S1 k rho1 rho2 ->
+    preord_env_P (Union var S1 (Union var (name_in_fundefs B1) (name_in_fundefs B2)))
+                 k (def_funs B1 B1 (def_funs B2 B2 rho1 rho1) (def_funs B2 B2 rho1 rho1))
+                 (def_funs B2 B2 (def_funs B1 B1 rho2 rho2) (def_funs B1 B1 rho2 rho2)).
+  Proof.
+    intros Hclo1 Hclo2 HD Hpre. rewrite (@Union_Setminus _ _ _ _).
+    apply preord_env_P_union.
+    - eapply preord_env_P_def_funs_not_in_P_r;
+      eauto using Disjoint_Setminus, Included_Union_r, Included_Union_l.
+      eapply preord_env_P_def_funs_not_in_P_l;
+        eauto using Disjoint_Setminus, Included_Union_r, Included_Union_l. 
+      eapply preord_env_P_def_funs_not_in_P_r;
+        eauto using Disjoint_Setminus, Included_Union_r, Included_Union_l.
+      eapply preord_env_P_def_funs_not_in_P_l;
+        eauto using Disjoint_Setminus, Included_Union_r, Included_Union_l.
+      eapply preord_env_P_antimon. eauto.
+      apply Subset_Setminus.
+    - apply preord_env_P_union.
+      + apply preord_env_P_def_funs_not_in_P_r; eauto.
+        eapply preord_env_P_def_funs_col.
+        eapply preord_env_P_antimon. apply preord_env_Empty_set.
+        intros x' HIn. inv HIn. exfalso. inv H. contradiction.
+        eapply Hclo1; eauto.
+      + apply preord_env_P_def_funs_not_in_P_l; eauto using Disjoint_sym.
+        eapply preord_env_P_def_funs_col.
+        eapply preord_env_P_antimon. apply preord_env_Empty_set.
+        intros x' HIn. inv HIn. exfalso. inv H. contradiction.
+        eapply Hclo2; eauto.
+  Qed.
+
+  Lemma preord_env_P_def_funs_strengthen_l (k : nat) rho rho' B1 B1' B2 :
+    Disjoint var (occurs_free_fundefs B1') (name_in_fundefs B2) ->
+    Disjoint var (name_in_fundefs B1') (name_in_fundefs B2) ->
+    closed_fundefs B1' ->
+    preord_env_P (name_in_fundefs B1) k
+                 (def_funs B1' B1 rho rho')
+                 (def_funs (fundefs_append B2 B1') B1 rho rho').
+  Proof.
+    revert rho rho' B1 B1' B2.
+    induction k as [ k IH' ] using lt_wf_rec1. intros rho rho' B1 B1' B2 HD1 HD2 Hclo.
+    induction B1.
+    - simpl. apply preord_env_P_extend.
+      + eapply preord_env_P_antimon. eapply IHB1; eauto.
+        rewrite Setminus_Union_distr, Setminus_Empty_set, Union_Empty_set_r.
+        eapply Setminus_Included. eapply Included_refl.
+      + rewrite preord_val_eq.
+        intros vs1 vs2 j t1 xs1 e1 rho1' Hlen Hf Hs.
+        edestruct setlist_length as [rho2' Hs']; eauto.
+        exists t1. exists xs1. exists e1. exists rho2'. split; eauto.
+        specialize (find_def_name_in_fundefs _ _ _ Hf); intros Hname.
+        destruct (@Dec _ _  (Decidable_name_in_fundefs B2) v).
+        exfalso. inv HD2. eapply H0; eauto.
+        eapply name_not_in_fundefs_find_def_None in H.
+        erewrite find_def_fundefs_append_r; eauto.
+        split. eauto. intros Hleq Hpre'.
+        eapply preord_exp_refl. 
+        eapply preord_env_P_setlist_l; [| | eauto | eauto | eauto].
+        rewrite def_funs_append.
+        apply preord_env_P_def_funs_not_in_P_r; eauto. 
+        intros x Hin Hfr.
+        apply find_def_correct in Hf.  
+        edestruct (occurs_free_in_fun _ _ _ _ _ Hf x Hfr); try contradiction.
+        inv H; eauto. unfold closed_fundefs in Hclo. rewrite Hclo in H0. inv H0.
+    - simpl. intros x HP. inv HP.
+  Qed.
+
+  
+  Lemma preord_val_def_funs_append_pre (k : nat) f tau xs e (B1 B2 : fundefs)
+        (rho1 rho2  : env) :
+    closed_fundefs (Fcons f tau xs (Efun B2 e) B1) ->
+    closed_fundefs B2 ->
+    unique_bindings_fundefs (Fcons f tau xs (Efun B2 e) B1) ->
+    Disjoint var (name_in_fundefs (Fcons f tau xs e B1)) (name_in_fundefs B2) ->
+    (forall j S1 rho1 rho2 rho1' rho2',
+       j < k ->
+       preord_env_P S1 j rho1 rho2 ->
+       preord_env_P (Union var S1 (name_in_fundefs B1))
+                    j (def_funs (Fcons f tau xs (Efun B2 e) B1) B1 rho1' rho1)
+                    (def_funs (fundefs_append (Fcons f tau xs e B1) B2) B1 rho2' rho2)) ->
+    preord_val k (Vfun rho1 (Fcons f tau xs (Efun B2 e) B1) f)
+               (Vfun rho2 (fundefs_append (Fcons f tau xs e B1) B2) f).
+  Proof.
+    revert f tau xs e B1 B2 rho1 rho2. induction k using lt_wf_rec1.
+    intros f tau xs e B1 B2 rho1 rho2 Hcl1 Hcl2 Hun HD Hyp. rewrite preord_val_eq.
+    intros vs1 vs2 j t1 xs1 e1 rho1' Hlen Hf Hs.
+    edestruct setlist_length as [rho2' Hs']; eauto. simpl in Hf.
+    destruct (M.elt_eq f f); try congruence. inv Hf. do 4 eexists. split. simpl.
+    destruct (M.elt_eq f f); try congruence. eauto. split; eauto.
+    intros Hleq Hpre'. simpl in Hs, Hs'. rewrite def_funs_append in Hs'.
+    intros v1 c1 Hleq1 Hstep1. inv Hstep1. edestruct preord_exp_refl; eauto.
+    apply preord_env_P_antimon with
+    (P2 := Union var (FromList xs1)
+                 (Union var (name_in_fundefs B2)
+                        (Union var (Singleton var f) (name_in_fundefs B1)))).
+    - repeat apply preord_env_P_union.
+      + apply preord_env_P_def_funs_not_in_P_l.
+        * eapply preord_env_P_setlist_l with (P1 := Empty_set var); eauto.
+          eapply preord_env_Empty_set. intros x Hc1 Hc2. exfalso; eauto.
+        * inv Hun. eapply Disjoint_Included_r.
+          eapply name_in_fundefs_bound_var_Efun. eauto using Disjoint_sym.
+      + eapply preord_env_P_setlist_not_in_P_r; eauto.
+        * eapply preord_env_P_set_not_in_P_r; eauto.
+          eapply preord_env_P_def_funs_not_in_P_r; eauto.
+          eapply preord_env_P_trans;
+            [| intros m; eapply preord_env_P_def_funs_strengthen_l
+               with (B2 := Fcons f t1 xs1 e B1); eauto ].
+          eapply preord_env_P_def_funs_col; eauto.
+          eapply preord_env_P_antimon. eapply preord_env_Empty_set.
+          rewrite Setminus_Empty_set. rewrite Union_Empty_set_r. apply Hcl2.
+          unfold closed_fundefs in Hcl2. rewrite Hcl2.
+          eapply Disjoint_Empty_set_l.
+          apply Disjoint_sym; eauto.
+          apply Disjoint_sym. eapply Disjoint_Union_r; eauto.
+          apply Disjoint_sym. eapply Disjoint_Union_l; eauto.
+        * inv Hun. eapply Disjoint_Included_l ; [| apply H8 ].
+          eapply name_in_fundefs_bound_var_Efun.
+      + eapply preord_env_P_setlist_not_in_P_r; eauto.
+        * eapply preord_env_P_def_funs_not_in_P_l; eauto.
+          eapply preord_env_P_setlist_not_in_P_l; eauto.
+          eapply preord_env_P_extend. rewrite Setminus_Empty_set.
+          eapply preord_env_Empty_set. 
+          eapply H; eauto. intros. eapply Hyp; eauto. omega.
+          inv Hun. constructor. intros x Hin. inv Hin. inv H0. contradiction.
+          inv Hun. eapply Disjoint_sym. eapply Disjoint_Singleton.
+          intros Hc. apply H6. apply name_in_fundefs_bound_var_Efun; eauto.
+        * inv Hun. apply Disjoint_sym. eapply Disjoint_Singleton; eauto.
+      + eapply preord_env_P_setlist_not_in_P_r; eauto.
+        * eapply preord_env_P_set_not_in_P_r; eauto.
+          eapply preord_env_P_def_funs_not_in_P_l; eauto.
+          eapply preord_env_P_setlist_not_in_P_l; eauto.
+          eapply preord_env_P_set_not_in_P_l; eauto.
+          eapply preord_env_P_antimon. eapply Hyp. omega.
+          eapply preord_env_Empty_set. rewrite Union_Empty_set_r.
+          eapply Included_refl.
+          inv Hun. eapply Disjoint_Singleton. intros Hc. apply H7.
+          apply name_in_fundefs_bound_var_fundefs; eauto.
+          inv Hun. eapply Disjoint_Included_l; [| apply H9 ].
+          apply name_in_fundefs_bound_var_fundefs; eauto.
+          eapply Disjoint_Union_r; eauto.
+          inv Hun. eapply Disjoint_Singleton. intros Hc. apply H7.
+          apply name_in_fundefs_bound_var_fundefs; eauto.
+        * inv Hun. eapply Disjoint_Included_l; [| apply H9 ]. intros x Hx. 
+          eapply name_in_fundefs_bound_var_fundefs; eauto.
+    - eapply Included_trans. eapply occurs_free_Efun_Included with (B := B2).
+      intros x Hfr. inv Hfr; eauto.
+      assert (Hin : fun_in_fundefs (Fcons f t1 xs1 (Efun B2 e) B1)
+                                   (f, t1, xs1, (Efun B2 e)))
+        by (constructor; eauto).
+      edestruct (occurs_free_in_fun _ _ _ _ _ Hin x H0); eauto.  inv H1; eauto.
+      unfold closed_fundefs in Hcl1. rewrite Hcl1 in H2. inv H2.
+  Qed.
+
+  Lemma preord_env_P_def_funs_append (k : nat) S1 f tau xs e (B1 B1' B2 : fundefs)
+        (rho1 rho2 rho1' rho2' : env) :
+    closed_fundefs (Fcons f tau xs (Efun B2 e) B1) ->
+    closed_fundefs B2 ->
+    unique_bindings_fundefs (Fcons f tau xs (Efun B2 e) B1) ->
+    Disjoint var (name_in_fundefs (Fcons f tau xs e B1)) (name_in_fundefs B2) ->
+    preord_env_P S1 k rho1 rho2 ->
+    preord_env_P (Union var S1 (name_in_fundefs B1'))
+                 k (def_funs (Fcons f tau xs (Efun B2 e) B1) B1' rho1' rho1)
+                 (def_funs (fundefs_append (Fcons f tau xs e B1) B2) B1' rho2' rho2).
+  Proof.
+    revert S1 f tau xs e B1 B1' B2 rho1 rho2 rho1' rho2'. induction k using lt_wf_rec1.
+    intros S1 f tau xs e B1 B1' B2 rho1 rho2 rho1' rho2' Hcl1 Hcl2 Hun HD Hpre1. simpl.
+    induction B1'.
+    - simpl. apply preord_env_P_extend.
+      + eapply preord_env_P_antimon. eauto.
+        rewrite !Setminus_Union_distr, Setminus_Empty_set, Union_Empty_set_r.
+        apply Included_Union_compat; eapply Setminus_Included; eapply Included_refl.
+      + destruct (M.elt_eq v f); subst.
+        * eapply preord_val_def_funs_append_pre; eauto.
+        * rewrite preord_val_eq. intros vs1 vs2 j t1 xs1 e1 rho1'' Hlen Hf Hs.
+          edestruct setlist_length as [rho2'' Hs']; [eauto | | ]. eauto.
+          exists t1, xs1, e1, rho2''. repeat split; eauto.
+          simpl in *. destruct (M.elt_eq v f); try congruence.
+          specialize (find_def_name_in_fundefs _ _ _ Hf); intros Hname.
+          erewrite <- find_def_fundefs_append_l in Hf; eauto.
+          intros Hleq Hpre'. eapply preord_exp_refl; eauto.
+          eapply preord_env_P_setlist_l with
+          (P1 := Union var (name_in_fundefs B1) (Singleton var f)); [| | eauto | eauto | eauto].
+          simpl. eapply preord_env_P_extend. eapply preord_env_P_antimon.
+          rewrite def_funs_append. eapply H; eauto. eapply preord_env_Empty_set.
+          rewrite Setminus_Union_distr, Setminus_Empty_set, Union_Empty_set_l, Union_Empty_set_r.
+          apply Setminus_Included. eapply Included_refl.
+          eapply preord_val_def_funs_append_pre; eauto. intros; eauto.
+          eapply H; eauto. omega.
+          destruct (M.elt_eq v f); try congruence. 
+          apply find_def_correct in Hf.
+          intros x Hin Hfr. specialize (occurs_free_in_fun _ _ _ _ _ Hf x Hfr).
+          intros H1. inv H1; try contradiction.
+          inv H0; eauto. simpl in H1. inv H1; eauto. right; eauto. left; eauto.
+          destruct (var_dec f x); subst. right; eauto.  
+          exfalso. eapply not_In_Empty_set. eapply Hcl1; eauto.
+    - simpl. now rewrite Union_Empty_set_l.
+  Qed.
+
+  Lemma preord_env_P_def_funs_hoist (k : nat) S1 f tau xs e (B1 B2 : fundefs)
+        (rho1 rho2 : env) :
+    closed_fundefs (Fcons f tau xs (Efun B2 e) B1) ->
+    closed_fundefs B2 ->
+    unique_bindings_fundefs (Fcons f tau xs (Efun B2 e) B1) ->
+    Disjoint var S1 (name_in_fundefs B2) ->
+    Disjoint var (name_in_fundefs (Fcons f tau xs e B1)) (name_in_fundefs B2) ->
+    preord_env_P S1 k rho1 rho2 ->
+    preord_env_P (Union var S1 (Union var (name_in_fundefs B1) (Singleton var f)))
+                 k (def_funs (Fcons f tau xs (Efun B2 e) B1)
+                             (Fcons f tau xs (Efun B2 e) B1)
+                             rho1 rho1)
+                 (def_funs (fundefs_append (Fcons f tau xs e B1) B2)
+                           (fundefs_append (Fcons f tau xs e B1) B2)
+                           rho2 rho2).
+  Proof.
+    intros Hcl1 Hcl2 Hun HD1 HD2 Hpre. simpl.
+    eapply preord_env_P_extend.
+    - eapply preord_env_P_antimon. 
+      rewrite def_funs_append. eapply preord_env_P_def_funs_append with (S1 := S1); eauto.
+      eapply preord_env_P_def_funs_not_in_P_r; eauto.
+      rewrite !Setminus_Union_distr, Setminus_Empty_set, Union_Empty_set_l.
+      eapply Included_Union_compat; apply Setminus_Included; apply Included_refl.
+    - eapply preord_val_def_funs_append_pre; eauto.
+      intros. eapply preord_env_P_def_funs_append; eauto.
+  Qed.
+
+  Lemma proerd_env_P_def_funs_weakening k S1 B B1 B2 f tau xs e rho rho':
+    ~ In var S1 f ->
+    preord_env_P S1 k (def_funs B (fundefs_append B1 B2) rho rho')
+                 (def_funs B (fundefs_append B1 (Fcons f tau xs e B2)) rho rho').
+  Proof.
+    revert S1 rho'. induction B1; intros S1 rho' Hin; simpl.
+    - destruct (var_dec f v); subst.
+      + apply preord_env_P_set_not_in_P_l; eauto using Disjoint_Singleton.
+        apply preord_env_P_set_not_in_P_r; eauto using Disjoint_Singleton.
+      + apply preord_env_P_extend. 
+        * eapply IHB1. intros Hc. inv Hc. eauto.
+        * eapply preord_val_refl.
+    - apply preord_env_P_set_not_in_P_r; eauto using Disjoint_Singleton.
+      apply preord_env_P_refl.
+  Qed.
+
+  (* TODO : make this a corollary of a following proof *)
+  Lemma preord_env_P_split_fds k S1 B1 B1' B2 B2' B11 B12 B11' B12' rho1 rho1' :
+    split_fds B11 B12 B1 ->
+    split_fds B11' B12' B1' ->
+    split_fds B11 B12 B2 ->
+    split_fds B11' B12' B2' ->
+    unique_bindings_fundefs B1' ->
+    unique_bindings_fundefs B1 ->  
+    preord_env_P S1 k (def_funs B1' B1 rho1 rho1') (def_funs B2' B2 rho1 rho1').
+  Proof.
+    intros Hspl.
+    revert B1 B11 B12 Hspl S1 B1' B2 B2' B11' B12' rho1 rho1'. induction k using lt_wf_rec1.
+    induction B1; intros B11 B12 Hspl1 S1 B1' B2 B2' B11' B12' rho1 rho1'
+                         Hspl1' Hspl2 Hspl2' Hun1 Hun2.
+    - edestruct split_fds_unique_bindings_fundefs_l as [H1 [H2 H3]]; [| |]; eauto.
+      specialize (split_fds_unique_bindings_fundefs_r _ _ _ H1 H2 H3 Hspl2); intros H4.
+      inv Hspl1.
+      + edestruct split_fds_cons_l_append_fundefs as [B3 [B4 [Heq Hspl3]]]; eauto.
+        eapply preord_env_P_antimon;
+          [| apply (@Included_Union_Setminus _ _ (name_in_fundefs B2) _)].
+        eapply preord_env_P_union.
+        * eapply preord_env_P_def_funs_not_in_P_r;
+          eauto using Disjoint_Setminus, Included_refl.
+          eapply preord_env_P_def_funs_not_in_P_l. eapply preord_env_P_refl.
+          rewrite split_fds_name_in_fundefs; eauto. simpl.
+          rewrite split_fds_name_in_fundefs with (B3 := B1); eauto.
+          rewrite Union_assoc. apply Disjoint_Setminus. apply Included_refl.
+        * rewrite split_fds_name_in_fundefs; eauto. simpl (Union _ _ _).
+          rewrite <- Union_assoc.
+          eapply preord_env_P_union.
+          rewrite Heq. rewrite def_funs_append; eauto.
+          eapply preord_env_P_def_funs_not_in_P_r.
+          simpl. apply preord_env_P_extend.
+          rewrite Setminus_Empty_set. apply preord_env_Empty_set.
+          { rewrite preord_val_eq. intros vs1 vs2 j t1 xs1 e1 rho1'' Hlen Hf Hs.
+            edestruct setlist_length as [rho2'' Hs']; [eauto | | ]. eauto.
+            exists t1, xs1, e1, rho2''. repeat split; eauto.
+            erewrite <- find_def_split_fds; eauto.
+            intros Hleq Hpre'. eapply preord_exp_refl; eauto.
+            eapply preord_env_P_setlist_l; [| | | eauto | eauto ]; eauto. }
+          symmetry in Heq. eapply fundefs_append_split_fds in Heq.
+          edestruct split_fds_unique_bindings_fundefs_l as [H5 [H6 H8]]. apply H4.  eauto.
+          rewrite bound_var_fundefs_Fcons in H8. apply Disjoint_sym in H8.
+          eapply Disjoint_Union_l. eapply Disjoint_Included_r; eauto.
+          eapply name_in_fundefs_bound_var_fundefs.
+          simpl. eapply preord_env_P_set_not_in_P_l.
+          rewrite Heq. eapply preord_env_P_trans;
+            [| intros m; apply proerd_env_P_def_funs_weakening ].
+          eapply IHB1; eauto. inv Hun2; eauto.
+          edestruct split_fds_unique_bindings_fundefs_l as [H5 [H6 H8]]; [apply H4| |]; eauto.
+          intros Hc. inv H5. inv Hc; eauto. apply H14.
+          apply name_in_fundefs_bound_var_fundefs; eauto.
+          eapply H8. constructor. rewrite bound_var_fundefs_Fcons. left; eauto.
+          apply name_in_fundefs_bound_var_fundefs; eauto.
+          inv H1. apply Disjoint_Singleton. intros Hc. inv Hc.
+          eapply H11. apply name_in_fundefs_bound_var_fundefs; eauto.
+          eapply H3. constructor. rewrite bound_var_fundefs_Fcons. left; eauto.
+          apply name_in_fundefs_bound_var_fundefs; eauto.
+      + edestruct split_fds_cons_r_append_fundefs as [B3 [B4 [Heq Hspl3]]]; eauto.
+        eapply preord_env_P_antimon;
+          [| apply (@Included_Union_Setminus _ _ (name_in_fundefs B2) _)].
+        eapply preord_env_P_union.
+        * eapply preord_env_P_def_funs_not_in_P_r;
+          eauto using Disjoint_Setminus, Included_refl.
+          eapply preord_env_P_def_funs_not_in_P_l. eapply preord_env_P_refl.
+          rewrite split_fds_name_in_fundefs; eauto. simpl.
+          rewrite split_fds_name_in_fundefs with (B3 := B1); eauto.
+          rewrite !Union_assoc. rewrite (Union_sym (Singleton var v)).
+          apply Disjoint_Setminus. apply Included_refl.
+        * rewrite split_fds_name_in_fundefs; eauto. simpl (Union _ _ _).
+          rewrite Union_assoc, (Union_sym _ (Singleton var v)), <- Union_assoc.
+          eapply preord_env_P_union.
+          rewrite Heq. rewrite def_funs_append; eauto.
+          eapply preord_env_P_def_funs_not_in_P_r.
+          simpl. apply preord_env_P_extend.
+          rewrite Setminus_Empty_set. apply preord_env_Empty_set.
+          { rewrite preord_val_eq. intros vs1 vs2 j t1 xs1 e1 rho1'' Hlen Hf Hs.
+            edestruct setlist_length as [rho2'' Hs']; [eauto | | ]. eauto.
+            exists t1, xs1, e1, rho2''. repeat split; eauto.
+            erewrite <- find_def_split_fds; eauto.
+            intros Hleq Hpre'. eapply preord_exp_refl; eauto.
+            eapply preord_env_P_setlist_l; [| | | eauto | eauto ]; eauto. }
+          symmetry in Heq. eapply fundefs_append_split_fds in Heq.
+          edestruct split_fds_unique_bindings_fundefs_l as [H5 [H6 H8]].
+          apply H4. eauto.
+          rewrite bound_var_fundefs_Fcons in H8. apply Disjoint_sym in H8.
+          eapply Disjoint_Union_l. eapply Disjoint_Included_r; eauto.
+          eapply name_in_fundefs_bound_var_fundefs.
+          simpl. eapply preord_env_P_set_not_in_P_l.
+          rewrite Heq. eapply preord_env_P_trans;
+            [| intros m; apply proerd_env_P_def_funs_weakening ].
+          eapply IHB1; eauto. inv Hun2; eauto.
+          edestruct split_fds_unique_bindings_fundefs_l as [H5 [H6 H8]]; [apply H4| |]; eauto.
+          intros Hc. inv H6. inv Hc; eauto. eapply H8. constructor; eauto.
+          now apply name_in_fundefs_bound_var_fundefs; eauto.
+          eapply H14. now apply name_in_fundefs_bound_var_fundefs; eauto.
+          inv H2. apply Disjoint_Singleton. intros Hc. inv Hc.
+          eapply H3. constructor. now apply name_in_fundefs_bound_var_fundefs; eauto.
+          rewrite bound_var_fundefs_Fcons. left; eauto.
+          eapply H11. now apply name_in_fundefs_bound_var_fundefs; eauto.
+    - inv Hspl1. simpl. inv Hspl2. eapply preord_env_P_refl.
+  Qed.
+
+  Lemma preord_env_P_Included_fun_in_fundefs k B1 B1' B2 B2' rho1 rho1' :
+    Included _ (fun_in_fundefs B1) (fun_in_fundefs B2) ->
+    Included _ (fun_in_fundefs B1') (fun_in_fundefs B2') ->
+    closed_fundefs B1' ->
+    unique_bindings_fundefs B1'->
+    unique_bindings_fundefs B1 ->
+    unique_bindings_fundefs B2'->
+    unique_bindings_fundefs B2 ->
+    preord_env_P (name_in_fundefs B1) k (def_funs B1' B1 rho1 rho1')
+                 (def_funs B2' B2 rho1 rho1').
+  Proof.
+    revert B1 B1' B2 B2' rho1 rho1'. induction k using lt_wf_rec1.
+    induction B1; intros B1' B2 B2' rho1 rho1' HS1 HS2 Hcl Hun1' Hun1 Hun2' Hun2.
+    - edestruct fun_in_fundefs_unique_bindings_split
+      with (B := B2) as [B [B' [Heq [Hn [HS Hun']]]]]; eauto.
+      eapply HS1. left. eauto.
+      edestruct fundefs_append_unique_bindings_l as [H1 [H2 H3]]; eauto.
+      rewrite Heq.
+      eapply preord_env_P_antimon;
+        [| apply (@Included_Union_Setminus _ _ (Singleton var v) _)].
+      eapply preord_env_P_union.
+      + simpl. eapply preord_env_P_set_not_in_P_l;
+          eauto using Disjoint_Setminus,  Included_refl.
+        eapply preord_env_P_trans;
+          [| intros m; apply proerd_env_P_def_funs_weakening; intros Hc; inv Hc; eauto ].
+        rewrite Setminus_Union_distr, Setminus_Empty_set, Union_Empty_set_r.
+        eapply preord_env_P_antimon; [ eapply IHB1; eauto |].
+        rewrite (fundefs_append_fun_in_fundefs B B' (fundefs_append B B')); eauto.
+        rewrite HS. simpl in HS1.
+        rewrite <- (Setminus_Disjoint (fun_in_fundefs B1) (Singleton _ (v, t, l, e))).
+        rewrite <- Setminus_Union_Inlcluded; eauto using Included_refl.
+        eapply Included_Setminus_compat; eauto using Included_refl.
+        now rewrite Union_sym.  
+        eapply Disjoint_Singleton. inv Hun1; eauto. intros Hc. apply H9.
+        apply name_in_fundefs_bound_var_fundefs.
+        now eapply fun_in_fundefs_name_in_fundefs; eauto.
+        now inv Hun1; eauto.
+        apply Setminus_Disjoint. eapply Disjoint_Singleton. inv Hun1; eauto.
+        intros Hc. apply H9. now apply name_in_fundefs_bound_var_fundefs; eauto.
+      + rewrite def_funs_append;
+        eapply preord_env_P_def_funs_not_in_P_r.
+        * simpl. eapply preord_env_P_extend.
+          rewrite Setminus_Empty_set. apply preord_env_Empty_set.
+          rewrite preord_val_eq. intros vs1 vs2 j t1 xs1 e1 rho1'' Hlen Hf Hs. 
+          edestruct setlist_length as [rho2'' Hs']; [eauto | | ]. eauto.
+          exists t1, xs1, e1, rho2''. repeat split; eauto.
+          erewrite <- find_def_Included_fun_in_fundefs; eauto.
+          eapply fun_in_fundefs_name_in_fundefs. now eapply find_def_correct; eauto.
+          intros Hleq Hpre'. eapply preord_exp_refl; eauto. 
+          eapply preord_env_P_setlist_l; [| | | eauto | eauto ]; eauto.
+          intros c Hnin Hf'. apply find_def_correct in Hf.
+          eapply occurs_free_in_fun in Hf'; eauto. inv Hf'.
+          exfalso; eauto. inv H0; eauto.
+          exfalso. eapply not_In_Empty_set. eapply Hcl; eauto.
+        * apply Disjoint_sym. apply Disjoint_Singleton. eauto.
+    - simpl. eapply preord_env_Empty_set.
+  Qed.
+
+  Lemma preord_env_P_def_funs_merge k S1 B B' B'' rho rho' :
+    unique_bindings_fundefs B ->
+    split_fds B' B'' B ->
+    closed_fundefs B' ->
+    closed_fundefs B'' ->
+    preord_env_P S1 k rho rho' ->
+    preord_env_P (Union var S1 (name_in_fundefs B)) k
+                 (def_funs B' B' (def_funs B'' B'' rho rho)
+                           (def_funs B'' B'' rho rho))
+                 (def_funs B B rho' rho').
+  Proof.
+    intros Hun HS Hcl Hcl' Hpre.
+    assert (Hcl'' := split_fds_closed_fundefs B' B'' B HS Hcl Hcl').
+    rewrite (@Union_Setminus _ _ _ _ ).
+    eapply preord_env_P_union.
+    - eapply preord_env_P_def_funs_not_in_P_l.
+      eapply preord_env_P_def_funs_not_in_P_l.
+      eapply preord_env_P_def_funs_not_in_P_r.
+      eapply preord_env_P_antimon; eauto.
+      apply Subset_Setminus.
+      apply Disjoint_Setminus; eauto using Included_refl.
+      eapply Disjoint_Setminus. 
+      rewrite !name_in_fundefs_big_cup_fun_in_fundefs.
+      eapply Included_big_cup. intros x; eauto using Same_set_refl.
+      rewrite (split_fds_fun_in_fundefs B' B'' B); eauto. now apply Included_Union_r.
+      edestruct split_fds_unique_bindings_fundefs_l as [H1 [H2 H3]]; eauto.
+      rewrite split_fds_name_in_fundefs; eauto.
+      eapply Disjoint_Setminus. eapply Included_Union_l.
+    - edestruct split_fds_unique_bindings_fundefs_l as [H1 [H2 H3]]; eauto.
+      rewrite split_fds_name_in_fundefs; eauto. eapply preord_env_P_union.
+      + eapply preord_env_P_trans.
+        eapply preord_env_P_Included_fun_in_fundefs with (B2 := B) (B2' := B);
+          eauto using Included_refl;
+          try (now rewrite (split_fds_fun_in_fundefs B' B'' B); eauto;
+               apply Included_Union_l).
+        intros m. eapply preord_env_P_def_funs_col.
+        rewrite (split_fds_name_in_fundefs B' B'' B); eauto.
+        unfold closed_fundefs in *. rewrite Hcl'', Union_Empty_set_l.
+        rewrite Setminus_Included_Empty_set. eapply preord_env_Empty_set.
+        eapply Included_Union_l.
+      + eapply preord_env_P_def_funs_not_in_P_l.
+        eapply preord_env_P_trans.
+        eapply preord_env_P_Included_fun_in_fundefs with (B2 := B) (B2' := B);
+          eauto using Included_refl;
+          try (now rewrite (split_fds_fun_in_fundefs B' B'' B); eauto;
+               apply Included_Union_r).
+        intros m. eapply preord_env_P_def_funs_col.
+        rewrite (split_fds_name_in_fundefs B' B'' B); eauto.
+        unfold closed_fundefs in *. rewrite Hcl'', Union_Empty_set_l.
+        rewrite Setminus_Included_Empty_set. eapply preord_env_Empty_set.
+        eapply Included_Union_r.
+        eapply Disjoint_Included_r. eapply name_in_fundefs_bound_var_fundefs.
+        eapply Disjoint_Included_l. eapply name_in_fundefs_bound_var_fundefs.
+        now apply Disjoint_sym.
+  Qed.
+
+  Lemma preord_env_P_Same_set_fun_in_fundefs k S1 B1 B1' B2 B2' rho1 rho1' :
+    Same_set _ (fun_in_fundefs B1) (fun_in_fundefs B2) ->
+    Same_set _ (fun_in_fundefs B1') (fun_in_fundefs B2') ->
+    unique_bindings_fundefs B1'->
+    unique_bindings_fundefs B1 ->
+    unique_bindings_fundefs B2'->
+    unique_bindings_fundefs B2 ->
+    preord_env_P S1 k (def_funs B1' B1 rho1 rho1') (def_funs B2' B2 rho1 rho1').
+  Proof. 
+    revert B1 S1 B1' B2 B2' rho1 rho1'. induction k using lt_wf_rec1.
+    induction B1; intros S1 B1' B2 B2' rho1 rho1' HS1 HS2 Hun1' Hun1 Hun2' Hun2.
+    - edestruct fun_in_fundefs_unique_bindings_split
+      with (B := B2) as [B [B' [Heq [Hn [HS Hun']]]]]; eauto.
+      eapply HS1. left. eauto.
+      edestruct fundefs_append_unique_bindings_l as [H1 [H2 H3]]; eauto.
+      rewrite Heq. 
+      eapply preord_env_P_antimon;
+        [| apply (@Included_Union_Setminus _ _ (Singleton var v) _)].
+      eapply preord_env_P_union.
+      + simpl. eapply preord_env_P_set_not_in_P_l;
+          eauto using Disjoint_Setminus, Included_refl.
+        eapply preord_env_P_trans;
+          [| intros m; apply proerd_env_P_def_funs_weakening; intros Hc; inv Hc; eauto ].
+        eapply IHB1; eauto ; try (now inv Hun1; eauto).
+        rewrite (fundefs_append_fun_in_fundefs B B' (fundefs_append B B')); eauto.
+        rewrite HS, <- HS1. simpl.
+        rewrite Setminus_Union_distr, Setminus_Empty_set, Union_Empty_set_r.
+        apply Same_set_sym. eapply Setminus_Disjoint. eapply Disjoint_Singleton.
+        inv Hun1; eauto. intros Hc. apply H9. apply name_in_fundefs_bound_var_fundefs.
+        eapply fun_in_fundefs_name_in_fundefs; eauto.
+      + rewrite def_funs_append;
+        eapply preord_env_P_def_funs_not_in_P_r.
+        * simpl. eapply preord_env_P_extend.
+          rewrite Setminus_Empty_set. apply preord_env_Empty_set.
+          rewrite preord_val_eq. intros vs1 vs2 j t1 xs1 e1 rho1'' Hlen Hf Hs. 
+          edestruct setlist_length as [rho2'' Hs']; [eauto | | ]. eauto.
+          exists t1, xs1, e1, rho2''. repeat split; eauto.
+          erewrite <- find_def_Same_set_fun_in_fundefs; eauto.
+          intros Hleq Hpre'. eapply preord_exp_refl; eauto.
+          eapply preord_env_P_setlist_l; [| | | eauto | eauto ]; eauto.
+        * apply Disjoint_sym. apply Disjoint_Singleton. eauto.
+    - simpl. destruct B2; eauto using preord_env_P_refl.
+      destruct HS1 as [_ H1]. exfalso. eapply not_In_Empty_set. eapply H1.
+      simpl. eauto.
+  Qed.
 
 (** step-indexed relation on cps terms. Relates
  * cps-terms with closure-converted terms  *)
@@ -27,8 +1716,8 @@ Fixpoint cc_approx_val (k : nat) (v1 v2 : val) {struct k} : Prop :=
       let '(e1, rho1) := p1 in
       let '(e2, rho2) := p2 in
       forall v1 c1,
-        c1 <= k -> bstep_e rho1 e1 v1 c1 ->
-        exists v2 c2, bstep_e rho2 e2 v2 c2 /\ 
+        c1 <= k -> bstep_e pr rho1 e1 v1 c1 ->
+        exists v2 c2, bstep_e pr rho2 e2 v2 c2 /\ 
                  cc_approx_val (k - c1) v1 v2
   in
   let fix cc_approx_val_aux (v1 v2 : val) {struct v1} : Prop :=
@@ -63,11 +1752,6 @@ Fixpoint cc_approx_val (k : nat) (v1 v2 : val) {struct k} : Prop :=
         | Vconstr tau1 t1 vs1, Vconstr tau2 t2 vs2 =>
           t1 = t2 /\ Forall2_aux vs1 vs2
         | Vint n1, Vint n2 => n1 = n2
-        | Vother t1, Vother t2 => True
-        (* XXX : Question.  *)
-        | Vobvs t1, Vobvs t2 => True
-        | Vobservable t1 vs1, Vobservable t2 vs2 =>
-          Forall2_aux vs1 vs2
         | _, _ => False
       end
   in cc_approx_val_aux v1 v2.
@@ -76,8 +1760,8 @@ Definition cc_approx_exp (k : nat) (p1 p2 : exp * env) : Prop :=
   let '(e1, rho1) := p1 in
   let '(e2, rho2) := p2 in
   forall v1 c1,
-    c1 <= k -> bstep_e rho1 e1 v1 c1 ->
-    exists v2 c2, bstep_e rho2 e2 v2 c2 /\
+    c1 <= k -> bstep_e pr rho1 e1 v1 c1 ->
+    exists v2 c2, bstep_e pr rho2 e2 v2 c2 /\
              cc_approx_val (k - c1) v1 v2.
 
 (** more compact definition of the value relation *)
@@ -99,10 +1783,6 @@ Definition cc_approx_val' (k : nat) (v1 v2 : val) : Prop :=
     | Vconstr tau1 t1 vs1, Vconstr tau2 t2 vs2 =>
       t1 = t2 /\ Forall2_asym (cc_approx_val k) vs1 vs2
     | Vint n1, Vint n2 => n1 = n2
-    | Vother t1, Vother t2 => True
-    | Vobvs t1, Vobvs t2 => True
-    | Vobservable t1 vs1, Vobservable t2 vs2 =>
-      Forall2_asym (cc_approx_val k) vs1 vs2
     | _, _ => False
   end.
 
@@ -128,12 +1808,6 @@ Proof.
     destruct l; try contradiction; destruct v1; try contradiction;
     intros; edestruct (Hpre vs1 vs2 0) as [t2' [Γ [xs2 [e2 [rho' [H1' [H2' H3']]]]]]];
     eauto; do 5 eexists; repeat split; eauto; intros Hc; exfalso; omega.
-  - revert l0; induction l as [| x xs IHxs];
-    intros l2; destruct l2 as [| y ys ];
-    split; intros H; try (now simpl in H; inv H); try now (simpl; eauto).
-    + destruct H as [H1 H2]; eauto.
-      constructor; eauto. eapply IHxs. eauto.
-    + inv H. split; eauto. eapply IHxs; eauto. 
   - split.
     * revert l0; induction l as [| x xs IHxs];
       intros l2; destruct l2 as [| y ys ];
@@ -153,12 +1827,6 @@ Proof.
     eauto; do 5 eexists; repeat split; eauto; intros Hleq Hf v1 c1 Hleq' Hstep;
     (assert (Heq : k - (k - j) = j) by omega);
     rewrite Heq in *;  eapply H3'; eauto.
-  - simpl; revert l0; induction l as [| x xs IHxs];
-    intros l2; destruct l2 as [| y ys ];
-    split; intros H; try (now simpl in H; inv H).
-    destruct H as [H1 H2]; eauto.
-    constructor; eauto. now eapply IHxs.
-    inv H. split; [now eauto | now apply IHxs].
 Qed.
 
 Opaque cc_approx_val.
@@ -425,9 +2093,6 @@ Proof.
     edestruct Hpre as [t2' [Γ [xs2 [e2 [rho2' [H1 [H2 H3]]]]]]]; eauto.
     do 5 eexists; split; eauto. split; eauto. intros Hleq' Hall. 
     eapply H3; eauto. omega.
-  - constructor.
-  - inv Hpre. constructor; rewrite cc_approx_val_eq in *. now eapply IHv1; eauto.
-    now eapply (IHv0 (Vobservable tau l')) in H3.
 Qed.
 
 (** The expression relation is monotonic in the step index *)
@@ -523,7 +2188,7 @@ Proof.
     repeat eexists; eauto. econstructor; eauto. simpl; rewrite Heq; eauto.
 Qed.
 
-Axiom Prim_axiom :
+Axiom Prim_axiom_cc :
   forall f f' v1,
     M.get f pr = Some f' ->
     forall k vs1 vs2,
@@ -543,42 +2208,14 @@ Lemma cc_approx_exp_prim_compat k rho1 rho2 x1 x2 tau f ys1 ys2 e1 e2 :
 Proof.
   intros Henv Hexp v1 c1 Hleq1 Hstep1. inv Hstep1.
   edestruct cc_approx_var_env_getlist as [vs2 [Hget' Hpre']]; eauto.
-  edestruct Prim_axiom as [v2 [Heq Hprev2]]; eauto.
+  edestruct Prim_axiom_cc as [v2 [Heq Hprev2]]; eauto.
   edestruct Hexp as [v2' [c2 [Hstepv2' Hprev2']]]; eauto.
   repeat eexists; eauto. econstructor; eauto.
 Qed.
 
-
 (** Lift a value predicate to a subset of an environment *)
 Definition lift_P_env (S : Ensemble var) (P : Ensemble val) (rho : env) :=
   forall x v, S x -> M.get x rho = Some v -> P v.
-
-(* TODO: move to identifiers.v *)
-Inductive closed_fundefs_in_val : val -> Prop :=
-| Vconstr_closed :
-    forall tau t vs,
-      Forall closed_fundefs_in_val vs ->
-      closed_fundefs_in_val (Vconstr tau t vs)
-| Vfun_closed :
-    forall rho B f,
-      closed_fundefs B ->
-      closed_fundefs_in_fundefs B ->
-      (* fun_in_fundefs B (f, tau, xs, e) -> *)
-      (* Included _ (occurs_free e) (Union _ (FromList xs) (name_in_fundefs B)) -> *)
-      closed_fundefs_in_val (Vfun rho B f)
-| Vint_closed :
-    forall z, closed_fundefs_in_val (Vint z)
-| Vother_closed :
-    forall tau, closed_fundefs_in_val (Vother tau)
-| Vobs :
-    forall tau, closed_fundefs_in_val (Vobvs tau)
-| Vobservable_closed :
-    forall tau vs,
-      Forall closed_fundefs_in_val vs ->
-      closed_fundefs_in_val (Vobservable tau vs).
-
-Definition closed_fundefs_in_env (S : Ensemble var) rho : Prop :=
-  lift_P_env S closed_fundefs_in_val rho.
 
 Lemma lift_P_env_antimon S S' P rho :
   Included _ S S' ->
@@ -705,94 +2342,6 @@ Proof.
   - eapply IHl; eauto.  
 Qed. 
 
-(* TODO: move to identifiers.v *)
-Lemma fun_in_fundefs_funs_in_fundef B B' f t xs e :
-  fun_in_fundefs B (f, t, xs, e) ->
-  funs_in_exp B' e ->
-  funs_in_fundef B' B.
-Proof.
-  induction B; intros Hin Hfuns.
-  - inv Hin.
-    + inv H. now eauto.
-    + constructor 2. eapply IHB; eauto.
-  - inv Hin.
-Qed.
-
-Axiom prims_closed_fundefs :
-  forall (f : prim) (f' : list val -> option val) vs v,
-    M.get f pr = Some f' ->
-    Forall closed_fundefs_in_val vs ->
-    f' vs = Some v ->
-    closed_fundefs_in_val v.
-
-Lemma bstep_e_preserves_closed_fundefs rho e v c :
-  bstep_e rho e v c ->
-  closed_fundefs_in_env (occurs_free e) rho ->
-  closed_fundefs_in_exp e ->
-  closed_fundefs_in_val v.
-Proof.
-  intros Hstep Hcl1 Hcl2. induction Hstep.
-  - constructor.
-    eapply lift_P_env_getlist; eauto.
-    rewrite occurs_free_Eapp. apply Included_Union_l.
-  - eapply IHHstep.
-    + subst. eapply lift_P_env_extend. 
-      * eapply lift_P_env_antimon; [| now eauto ].
-        rewrite occurs_free_Econstr.
-        eapply Included_Union_r.
-      * constructor. eapply lift_P_env_getlist; eauto.
-        rewrite occurs_free_Econstr. eapply Included_Union_l.
-    + intros B Hin. eauto.
-  - eapply IHHstep.
-    + subst. eapply lift_P_env_extend. 
-      * eapply lift_P_env_antimon; [| now eauto ].
-        rewrite occurs_free_Eproj.
-        eapply Included_Union_r.
-      * eapply Forall_nthN; [| eassumption ].
-        eapply lift_P_env_get in H; [| eassumption |].
-        now inv H. 
-        rewrite occurs_free_Eproj. eapply Included_Union_l.
-    + intros B Hin. eauto.
-  - eapply IHHstep.
-    + eapply lift_P_env_antimon; [| now eauto ].
-      eapply occurs_free_Ecase_Included.
-      eapply findtag_In_patterns. eassumption.
-    + intros B Hin. eapply Hcl2.
-      econstructor; eauto. apply findtag_In_patterns. eassumption.
-  - eapply IHHstep.
-    + eapply Hcl1 in H; [| now eauto ]. inv H.
-      apply find_def_correct in H1.  
-      eapply lift_P_env_antimon. eapply occurs_free_in_fun.
-      eassumption.
-      unfold closed_fundefs in H5. rewrite H5, Union_Empty_set_l.
-      eapply lift_P_env_setlist; [| | now eauto ].
-      * rewrite Setminus_Union_distr, Setminus_Empty_set, Union_Empty_set_r.
-        eapply  lift_P_env_def_funs.
-        rewrite Setminus_Included_Empty_set. now apply lift_P_env_Emtpy_set.
-        eapply Setminus_Included. now apply Included_refl.
-        intros f''. now constructor. 
-      * eapply lift_P_env_getlist; [ eassumption | | eassumption ].
-        rewrite occurs_free_Eapp. eapply Included_Union_l.
-    + intros B Hin.
-      eapply Hcl1 in H; [| now eauto ].
-      eapply find_def_correct in H1.
-      inv H. eapply H7. eapply fun_in_fundefs_funs_in_fundef; eassumption. 
-  - eapply IHHstep.
-    + eapply lift_P_env_def_funs.
-      * eapply lift_P_env_antimon; [| eassumption ].
-        rewrite occurs_free_Efun. eapply Included_Union_r.
-      * intros f. constructor. now eapply Hcl2.
-        intros B H. eapply Hcl2. now eauto.
-    + intros B Hin. eauto.
-  - eapply IHHstep.
-    + subst. eapply lift_P_env_extend. 
-      * eapply lift_P_env_antimon; [| now eauto ].
-        rewrite occurs_free_Eprim. eapply Included_Union_r.
-      * eapply prims_closed_fundefs; [ eassumption | | eassumption ].
-        eapply lift_P_env_getlist; [ eassumption | | eassumption ].
-        rewrite occurs_free_Eprim. eapply Included_Union_l.
-    + intros B Hin. eauto.
-Qed.
  
 Lemma cc_approx_exp_respects_preord_exp_r_pre (k : nat)
       (rho1 rho2 rho3 : env) (e1 e2 e3 : exp) :
@@ -887,29 +2436,111 @@ Proof.
   - destruct v2; try contradiction.
     destruct v3; try contradiction. inv Happrox.
     inv Hpre'. reflexivity.
-  - destruct v2; try contradiction.
-    destruct v3; try contradiction. inv Happrox.
-    inv Hpre'. reflexivity.
-  - destruct v2; try contradiction.
-    destruct v3; try contradiction. inv Happrox.
-    inv Hpre'. reflexivity.
-  - destruct v2; try contradiction.
-    destruct v3; try contradiction.
-    constructor.
-  - destruct v2; try contradiction.
-    destruct v3; try contradiction.
-    destruct l0; [now inv Happrox; inv H1 |].
-    destruct l1; [now inv Hpre'; inv H1 |].
-    inv Hpre'; inv Happrox.
-    constructor.
-    + eapply IHv1; [ now eauto |].
-      intros k'. specialize (Hpre k').
-      rewrite preord_val_eq in Hpre. now inv Hpre.
-    + assert (Hsuf : cc_approx_val' k (Vobservable tau l)  (Vobservable tau l1)).
-      { rewrite <- cc_approx_val_eq.
-        eapply IHv0 with (v2 := Vobservable tau l0); eauto.
-        - rewrite cc_approx_val_eq. now eauto.
-        - intros k'. specialize (Hpre k'). rewrite preord_val_eq in Hpre.
-          inv Hpre. now rewrite preord_val_eq. }
-      now eauto.
 Qed.
+
+(* The following are obsolete *)
+(* TODO: move to identifiers.v *)
+Inductive closed_fundefs_in_val : val -> Prop :=
+| Vconstr_closed :
+    forall tau t vs,
+      Forall closed_fundefs_in_val vs ->
+      closed_fundefs_in_val (Vconstr tau t vs)
+| Vfun_closed :
+    forall rho B f,
+      closed_fundefs B ->
+      closed_fundefs_in_fundefs B ->
+      (* fun_in_fundefs B (f, tau, xs, e) -> *)
+      (* Included _ (occurs_free e) (Union _ (FromList xs) (name_in_fundefs B)) -> *)
+      closed_fundefs_in_val (Vfun rho B f)
+| Vint_closed :
+    forall z, closed_fundefs_in_val (Vint z).
+
+Definition closed_fundefs_in_env (S : Ensemble var) rho : Prop :=
+  lift_P_env S closed_fundefs_in_val rho.
+
+Lemma fun_in_fundefs_funs_in_fundef B B' f t xs e :
+  fun_in_fundefs B (f, t, xs, e) ->
+  funs_in_exp B' e ->
+  funs_in_fundef B' B.
+Proof.
+  induction B; intros Hin Hfuns.
+  - inv Hin.
+    + inv H. now eauto.
+    + constructor 2. eapply IHB; eauto.
+  - inv Hin.
+Qed.
+
+Axiom prims_closed_fundefs :
+  forall (f : prim) (f' : list val -> option val) vs v,
+    M.get f pr = Some f' ->
+    Forall closed_fundefs_in_val vs ->
+    f' vs = Some v ->
+    closed_fundefs_in_val v.
+
+Lemma bstep_e_preserves_closed_fundefs rho e v c :
+  bstep_e pr rho e v c ->
+  closed_fundefs_in_env (occurs_free e) rho ->
+  closed_fundefs_in_exp e ->
+  closed_fundefs_in_val v.
+Proof.
+  intros Hstep Hcl1 Hcl2. induction Hstep.
+  - eapply IHHstep.
+    + subst. eapply lift_P_env_extend. 
+      * eapply lift_P_env_antimon; [| now eauto ].
+        rewrite occurs_free_Econstr.
+        eapply Included_Union_r.
+      * constructor. eapply lift_P_env_getlist; eauto.
+        rewrite occurs_free_Econstr. eapply Included_Union_l.
+    + intros B Hin. eauto.
+  - eapply IHHstep.
+    + subst. eapply lift_P_env_extend. 
+      * eapply lift_P_env_antimon; [| now eauto ].
+        rewrite occurs_free_Eproj.
+        eapply Included_Union_r.
+      * eapply Forall_nthN; [| eassumption ].
+        eapply lift_P_env_get in H; [| eassumption |].
+        now inv H. 
+        rewrite occurs_free_Eproj. eapply Included_Union_l.
+    + intros B Hin. eauto.
+  - eapply IHHstep.
+    + eapply lift_P_env_antimon; [| now eauto ].
+      eapply occurs_free_Ecase_Included.
+      eapply findtag_In_patterns. eassumption.
+    + intros B Hin. eapply Hcl2.
+      econstructor; eauto. apply findtag_In_patterns. eassumption.
+  - eapply IHHstep.
+    + eapply Hcl1 in H; [| now eauto ]. inv H.
+      apply find_def_correct in H1.  
+      eapply lift_P_env_antimon. eapply occurs_free_in_fun.
+      eassumption.
+      unfold closed_fundefs in H5. rewrite H5, Union_Empty_set_l.
+      eapply lift_P_env_setlist; [| | now eauto ].
+      * rewrite Setminus_Union_distr, Setminus_Empty_set, Union_Empty_set_r.
+        eapply  lift_P_env_def_funs.
+        rewrite Setminus_Included_Empty_set. now apply lift_P_env_Emtpy_set.
+        eapply Setminus_Included. now apply Included_refl.
+        intros f''. now constructor. 
+      * eapply lift_P_env_getlist; [ eassumption | | eassumption ].
+        rewrite occurs_free_Eapp. eapply Included_Union_l.
+    + intros B Hin.
+      eapply Hcl1 in H; [| now eauto ].
+      eapply find_def_correct in H1.
+      inv H. eapply H7. eapply fun_in_fundefs_funs_in_fundef; eassumption. 
+  - eapply IHHstep.
+    + eapply lift_P_env_def_funs.
+      * eapply lift_P_env_antimon; [| eassumption ].
+        rewrite occurs_free_Efun. eapply Included_Union_r.
+      * intros f. constructor. now eapply Hcl2.
+        intros B H. eapply Hcl2. now eauto.
+    + intros B Hin. eauto.
+  - eapply IHHstep.
+    + subst. eapply lift_P_env_extend. 
+      * eapply lift_P_env_antimon; [| now eauto ].
+        rewrite occurs_free_Eprim. eapply Included_Union_r.
+      * eapply prims_closed_fundefs; [ eassumption | | eassumption ].
+        eapply lift_P_env_getlist; [ eassumption | | eassumption ].
+        rewrite occurs_free_Eprim. eapply Included_Union_l.
+    + intros B Hin. eauto.
+Qed.
+
+End Log_rel.
